Escallon/LR_Parsing/LR0_Parser.thy
@@ -1373,23 +1373,23 @@ qed simp
 
   
 inductive stack_word :: "('n, 't) syms \<Rightarrow> ('n, 't) item set list \<times> 't list 
-  \<Rightarrow> ('n, 't) item set list \<times> 't list \<Rightarrow> bool" (\<open>_ \<Turnstile> _ \<turnstile>P* _\<close> 55)  where
-sw_refl [intro]: "[] \<Turnstile> c\<^sub>0 \<turnstile>P* c\<^sub>0" |
-sw_step: "\<lbrakk>\<alpha> \<Turnstile> c\<^sub>0 \<turnstile>P* (ps @ q # qs, u); (ps @ q # qs, u) \<turnstile>P (dfa.nxt LR\<^sub>0 q X # q # qs, v)\<rbrakk> 
-  \<Longrightarrow> X # drop (length ps) \<alpha> \<Turnstile> c\<^sub>0 \<turnstile>P* (dfa.nxt LR\<^sub>0 q X # q # qs, v)"
+  \<Rightarrow> ('n, 't) item set list \<times> 't list \<Rightarrow> bool" (\<open>_ \<turnstile> _ \<turnstile>P* _\<close> 55)  where
+sw_refl [intro]: "[] \<turnstile> c\<^sub>0 \<turnstile>P* c\<^sub>0" |
+sw_step: "\<lbrakk>\<alpha> \<turnstile> c\<^sub>0 \<turnstile>P* (ps @ q # qs, u); (ps @ q # qs, u) \<turnstile>P (dfa.nxt LR\<^sub>0 q X # q # qs, v)\<rbrakk> 
+  \<Longrightarrow> X # drop (length ps) \<alpha> \<turnstile> c\<^sub>0 \<turnstile>P* (dfa.nxt LR\<^sub>0 q X # q # qs, v)"
 
-inductive_cases stack_word_reflE [elim]: "[] \<Turnstile> c\<^sub>0 \<turnstile>P* c\<^sub>1"
-inductive_cases stack_word_stepE [elim]: "X # \<alpha> \<Turnstile> c\<^sub>0 \<turnstile>P* c\<^sub>1"
+inductive_cases stack_word_reflE [elim]: "[] \<turnstile> c\<^sub>0 \<turnstile>P* c\<^sub>1"
+inductive_cases stack_word_stepE [elim]: "X # \<alpha> \<turnstile> c\<^sub>0 \<turnstile>P* c\<^sub>1"
 
 lemma sw_stepI [intro]:
-  assumes "\<alpha> \<Turnstile> c\<^sub>0 \<turnstile>P* c\<^sub>1" "c\<^sub>1 \<turnstile>P c\<^sub>2"  
+  assumes "\<alpha> \<turnstile> c\<^sub>0 \<turnstile>P* c\<^sub>1" "c\<^sub>1 \<turnstile>P c\<^sub>2"  
     "c\<^sub>1 = (ps @ q # qs, u)" "c\<^sub>2 = (dfa.nxt LR\<^sub>0 q X # q # qs, v)" "\<alpha>' = drop (length ps) \<alpha>"
-  shows "X # \<alpha>' \<Turnstile> c\<^sub>0 \<turnstile>P* c\<^sub>2"
+  shows "X # \<alpha>' \<turnstile> c\<^sub>0 \<turnstile>P* c\<^sub>2"
   using assms sw_step by blast
 
 lemma sw_shift:
-  assumes "\<alpha> \<Turnstile> c\<^sub>0 \<turnstile>P* (ps, a # w)" "(ps, a # w) \<turnstile>P (qs, w)"
-  shows "Tm a # \<alpha> \<Turnstile> c\<^sub>0 \<turnstile>P* (qs, w)"
+  assumes "\<alpha> \<turnstile> c\<^sub>0 \<turnstile>P* (ps, a # w)" "(ps, a # w) \<turnstile>P (qs, w)"
+  shows "Tm a # \<alpha> \<turnstile> c\<^sub>0 \<turnstile>P* (qs, w)"
   using assms(2) proof cases
   case (shift r rs a w)
   from assms show ?thesis 
@@ -1397,26 +1397,26 @@ lemma sw_shift:
 qed simp_all
 
 lemma stack_word_imp_P0_steps:
-  "\<alpha> \<Turnstile> c\<^sub>0 \<turnstile>P* c\<^sub>1 \<Longrightarrow> c\<^sub>0 \<turnstile>P* c\<^sub>1"
+  "\<alpha> \<turnstile> c\<^sub>0 \<turnstile>P* c\<^sub>1 \<Longrightarrow> c\<^sub>0 \<turnstile>P* c\<^sub>1"
   by (induction rule: stack_word.induct) auto
 
 lemma P0_init_stack_word_length_inv:
-  "\<alpha> \<Turnstile> ([gpda.init P\<^sub>0], u) \<turnstile>P* (qs, v) \<Longrightarrow> Suc (length \<alpha>) = length qs"
+  "\<alpha> \<turnstile> ([gpda.init P\<^sub>0], u) \<turnstile>P* (qs, v) \<Longrightarrow> Suc (length \<alpha>) = length qs"
   by (induction "([gpda.init P\<^sub>0], u)" "(qs, v)" arbitrary: qs v rule: stack_word.induct) auto
 
 lemma P0_steps_imp_stack_word:
   assumes "c0 \<turnstile>P* (q # qs, w)" "q \<in> dfa.states LR\<^sub>0"
-  obtains \<alpha> where "\<alpha> \<Turnstile> c0 \<turnstile>P* (q # qs, w)"
+  obtains \<alpha> where "\<alpha> \<turnstile> c0 \<turnstile>P* (q # qs, w)"
   using assms proof (induction "(q # qs, w)" arbitrary: thesis q qs w)
   case (step c1)
   note that = step.prems
   note IH = step.hyps(3)
   from step(2) show ?case proof cases
     case (shift p ps a v)
-    with step obtain \<alpha> where sw: "\<alpha> \<Turnstile> c0 \<turnstile>P* ([] @ p # ps, a # w)" 
+    with step obtain \<alpha> where sw: "\<alpha> \<turnstile> c0 \<turnstile>P* ([] @ p # ps, a # w)" 
       by auto
     note step_unfolded = step[unfolded shift]
-    from sw have "Tm a # \<alpha> \<Turnstile> c0 \<turnstile>P* (q # qs, w)" unfolding shift
+    from sw have "Tm a # \<alpha> \<turnstile> c0 \<turnstile>P* (q # qs, w)" unfolding shift
       by standard (use step_unfolded shift(2) in auto)
     then show ?thesis using that by simp
   next
@@ -1424,17 +1424,17 @@ lemma P0_steps_imp_stack_word:
     from reduce(1,2) obtain ps' where c1_snoc: "c1 = (ps' @ p\<^sub>0 # rs, v)" 
       by (metis (no_types, lifting) append_Cons append_eq_append_conv2 list.distinct(1)
           snoc_eq_iff_butlast)
-    with reduce step obtain \<alpha> where sw: "\<alpha> \<Turnstile> c0 \<turnstile>P* (ps' @ p\<^sub>0 # rs, v)" 
+    with reduce step obtain \<alpha> where sw: "\<alpha> \<turnstile> c0 \<turnstile>P* (ps' @ p\<^sub>0 # rs, v)" 
       by (metis list.set_intros(1) subset_code(1))
     note step_unfolded = step[unfolded reduce(3-) c1_snoc]
-    from sw have "Nt X # drop (length ps') \<alpha> \<Turnstile> c0 \<turnstile>P* (q # qs, w)" unfolding reduce(3)
+    from sw have "Nt X # drop (length ps') \<alpha> \<turnstile> c0 \<turnstile>P* (q # qs, w)" unfolding reduce(3)
       by standard (use step_unfolded in simp_all)
     then show ?thesis using that by simp
   qed (use P0_final_item_notin_It in_state_imp_in_It that(2) in auto)
 qed fast
 
 lemma P0_nth_is_valids_of_nth_stack_word:
-  "\<alpha> \<Turnstile> ([gpda.init P\<^sub>0], u) \<turnstile>P* (q # qs, v) \<Longrightarrow> 
+  "\<alpha> \<turnstile> ([gpda.init P\<^sub>0], u) \<turnstile>P* (q # qs, v) \<Longrightarrow> 
     \<forall>n < length (q # qs). (q # qs) ! n  = valids (rev (drop n \<alpha>))"
 proof (induction "([gpda.init P\<^sub>0], u)" "(q # qs, v)" arbitrary: q qs u v rule: stack_word.induct)
   case (sw_step \<alpha> ps q qs v X w)
@@ -1482,7 +1482,7 @@ proof (induction "([gpda.init P\<^sub>0], u)" "(q # qs, v)" arbitrary: q qs u v 
 qed (use init_P0_is_valids_empty valids_def in force)
 
 lemma sw_last_is_init:
-  assumes "\<alpha> \<Turnstile> ([gpda.init P\<^sub>0], u) \<turnstile>P* (q # qs, v)"
+  assumes "\<alpha> \<turnstile> ([gpda.init P\<^sub>0], u) \<turnstile>P* (q # qs, v)"
   shows "last (q # qs) = gpda.init P\<^sub>0"
 proof -
   note len_qqs_Suc_len_\<alpha> = P0_init_stack_word_length_inv[OF assms]
@@ -1494,7 +1494,7 @@ proof -
 qed
 
 lemma sw_second_is_valids_tl:
-  assumes "\<alpha> \<Turnstile> ([gpda.init P\<^sub>0], u) \<turnstile>P* (p # q # qs, v)"
+  assumes "\<alpha> \<turnstile> ([gpda.init P\<^sub>0], u) \<turnstile>P* (p # q # qs, v)"
   shows "q = valids (rev (tl \<alpha>))"
 proof -
   note len_pqqs_Suc_len_\<alpha> = P0_init_stack_word_length_inv[OF assms]
@@ -1505,7 +1505,7 @@ proof -
 qed
 
 lemma P0_invariant1:
-  "\<lbrakk>\<alpha> \<Turnstile> ([gpda.init P\<^sub>0], u @ v) \<turnstile>P* (q # qs, v); q \<noteq> {}\<rbrakk> \<Longrightarrow> Prods G' \<turnstile> rev \<alpha> \<Rightarrow>r* map Tm u"
+  "\<lbrakk>\<alpha> \<turnstile> ([gpda.init P\<^sub>0], u @ v) \<turnstile>P* (q # qs, v); q \<noteq> {}\<rbrakk> \<Longrightarrow> Prods G' \<turnstile> rev \<alpha> \<Rightarrow>r* map Tm u"
 proof (induction "([gpda.init P\<^sub>0], u @ v)" "(q # qs, v)" arbitrary: q qs u v rule: stack_word.induct)
   case (sw_step \<alpha> ps q qs w X v)
   with stack_word_imp_P0_steps P0.reachable_imp_substring obtain u' where w_app: "u @ v = u' @ w"
@@ -1600,7 +1600,7 @@ qed
 
     Prods G' \<turnstile> \<alpha> \<Rightarrow>r* map Tm u \<Longrightarrow> (q\<^sub>0\<^sub>,\<^sub>M, u @ v) \<turnstile>M\<^sub>G* (\<alpha> @ [q\<^sub>0], v)
 
-    (q\<^sub>0\<^sub>,\<^sub>M, u @ v) \<turnstile>M\<^sub>G* (\<alpha> @ [q\<^sub>0], v) \<Longrightarrow> \<exists>qs. \<alpha> \<Turnstile> (q\<^sub>0\<^sub>,\<^sub>P, u @ v) \<turnstile>P* (valids \<alpha> # qs, v)
+    (q\<^sub>0\<^sub>,\<^sub>M, u @ v) \<turnstile>M\<^sub>G* (\<alpha> @ [q\<^sub>0], v) \<Longrightarrow> \<exists>qs. \<alpha> \<turnstile> (q\<^sub>0\<^sub>,\<^sub>P, u @ v) \<turnstile>P* (valids \<alpha> # qs, v)
     
  *)
 
@@ -1640,7 +1640,7 @@ qed (use dfa_LR0.init in simp)
 
 lemma MG_steps_imp_stack_word:
   assumes "([gpda.init M\<^sub>G], u) \<turnstile>M* (map Sym \<alpha> @ [gpda.init M\<^sub>G], v)" "valids (rev \<alpha>) \<noteq> {}"
-  obtains qs where "\<alpha> \<Turnstile> ([gpda.init P\<^sub>0], u) \<turnstile>P* (valids (rev \<alpha>) # qs, v)"
+  obtains qs where "\<alpha> \<turnstile> ([gpda.init P\<^sub>0], u) \<turnstile>P* (valids (rev \<alpha>) # qs, v)"
   using assms proof (induction "(map Sym \<alpha> @ [gpda.init M\<^sub>G], v)" arbitrary: \<alpha> v thesis rule: rtranclp_induct)
   case base
   then show ?case using base(2)[of "[]"] init_P0_is_valids_empty by force
@@ -1653,7 +1653,7 @@ next
       with shift step(1) have eq: 
         "(map Sym \<alpha> @ [gpda.init M\<^sub>G], v) = ([Sym (Tm a), gpda.init M\<^sub>G], w)" "u = a # w"
         using MG.reaches_Init_imp_refl by auto
-      have "[Tm a] \<Turnstile> ([gpda.init P\<^sub>0], a # w) \<turnstile>P* ([valids [Tm a], gpda.init P\<^sub>0], w)"
+      have "[Tm a] \<turnstile> ([gpda.init P\<^sub>0], a # w) \<turnstile>P* ([valids [Tm a], gpda.init P\<^sub>0], w)"
       proof (rule sw_shift)
         show "([gpda.init P\<^sub>0], a # w) \<turnstile>P ([valids [Tm a], gpda.init P\<^sub>0], w)" 
         proof
@@ -1672,9 +1672,9 @@ next
       with nempty_valids_imp_nempty_valids_prefix[] step(5) have 
         valids_\<beta>_nempty: "valids (rev \<beta>) \<noteq> {}" using \<alpha>_eq(1) by force
       with step(3)[OF c_eq(1)] obtain qs where sw_\<beta>:
-        "\<beta> \<Turnstile> ([gpda.init P\<^sub>0], u) \<turnstile>P* (valids (rev \<beta>) # qs, a # w)" 
+        "\<beta> \<turnstile> ([gpda.init P\<^sub>0], u) \<turnstile>P* (valids (rev \<beta>) # qs, a # w)" 
         by metis
-      hence "Tm a # \<beta> \<Turnstile> ([gpda.init P\<^sub>0], u) \<turnstile>P* (valids (rev \<alpha>) # valids (rev \<beta>) # qs, w)"
+      hence "Tm a # \<beta> \<turnstile> ([gpda.init P\<^sub>0], u) \<turnstile>P* (valids (rev \<alpha>) # valids (rev \<beta>) # qs, w)"
       proof (rule sw_shift)
         show "(valids (rev \<beta>) # qs, a # w) \<turnstile>P (valids (rev \<alpha>) # valids (rev \<beta>) # qs, w)"
         proof -
@@ -1702,9 +1702,9 @@ next
           using G_Prods_subset_G' by blast
       qed  
       with snoc reduce step(3)[of "rev \<beta> @ \<gamma>" w] obtain qs where sw_\<beta>\<gamma>:
-        "rev \<beta> @ \<gamma> \<Turnstile> ([gpda.init P\<^sub>0], u) \<turnstile>P* (valids (rev \<gamma> @ \<beta>) # qs, w)"
+        "rev \<beta> @ \<gamma> \<turnstile> ([gpda.init P\<^sub>0], u) \<turnstile>P* (valids (rev \<gamma> @ \<beta>) # qs, w)"
         using \<gamma>_def by auto
-      then have "Nt A # \<gamma> \<Turnstile> ([gpda.init P\<^sub>0], u) \<turnstile>P* (valids (rev \<gamma> @ [Nt A]) # drop (length \<beta>) (valids (rev \<gamma> @ \<beta>) # qs), w)"
+      then have "Nt A # \<gamma> \<turnstile> ([gpda.init P\<^sub>0], u) \<turnstile>P* (valids (rev \<gamma> @ [Nt A]) # drop (length \<beta>) (valids (rev \<gamma> @ \<beta>) # qs), w)"
       proof
         from A\<beta>_valid_for_\<gamma>\<beta>
         show "(valids (rev \<gamma> @ \<beta>) # qs, w) \<turnstile>P (valids (rev \<gamma> @ [Nt A]) # drop (length \<beta>) (valids (rev \<gamma> @ \<beta>) # qs), w)"
@@ -1759,8 +1759,6 @@ next
   qed (cases \<alpha>, auto)
 qed
 
-
-
 lemma P0_complete:
   "LangS G' \<subseteq> P0.Lang"
 proof
@@ -1772,7 +1770,7 @@ proof
   hence "([gpda.init P\<^sub>0], w) \<turnstile>P* ([valids [Nt S], gpda.init P\<^sub>0], [])"
   proof -
     obtain qs where
-      "[Nt S] \<Turnstile> ([gpda.init P\<^sub>0], w) \<turnstile>P* (valids [Nt S] # qs, [])" 
+      "[Nt S] \<turnstile> ([gpda.init P\<^sub>0], w) \<turnstile>P* (valids [Nt S] # qs, [])" 
     proof -
       have "valids (rev [Nt S]) \<noteq> {}" 
         by (metis (no_types, lifting) S'_complete_reliable_imp_S empty_iff in_states_imp_valid
