Escallon/LR_Parsing/thesis/Paper.thy
@@ -19,6 +19,9 @@ translations
 
 notation (latex output) drop (\<open>\<^bsub>_\<^esub>|_\<close>)
 
+notation (latex output) LangS (\<open>L'(_')\<close>)
+notation (latex output) gpda.Lang (\<open>L'(_')\<close>)
+
 abbreviation initial_item :: "'n \<Rightarrow> ('n,'t) syms \<Rightarrow> ('n,'t) item" ("[_ \<rightarrow>  \<cdot> _ ]") where
   "[A \<rightarrow> \<cdot> \<alpha> ] \<equiv>  [A \<rightarrow> [] \<cdot> \<alpha>]"
 abbreviation complete_item :: "'n \<Rightarrow> ('n,'t) syms \<Rightarrow> ('n,'t) item" ("[_ \<rightarrow> _ \<cdot> ]") where
@@ -42,37 +45,39 @@ text \<open>A term \<open>t\<close> of type \<open>\<tau>\<close> is notated as 
 is an example for this.\\
 The keyword \isakeyword{datatype} is used to declare algebraic data types, which can be seen in 
 @{typ "'a list"}:
-
+\begin{quote}
 @{datatype list}
+\end{quote}
 
-If \<open>xs = y # ys\<close>, \<open>hd xs = y\<close> and \<open>tl xs = ys\<close>. Furthermore, lists are concatenated with the operator 
+An explicit list can be either written as \<open>x\<^sub>0 # x\<^sub>1 # ... # x\<^sub>n\<close> or as \<open>[x\<^sub>0, x\<^sub>1, ..., x\<^sub>n]\<close>. If 
+\<open>xs = y # ys\<close>, \<open>hd xs = y\<close> and \<open>tl xs = ys\<close>. Furthermore, lists are concatenated with the operator 
 \<open>@\<close>, @{const rev} reverses a list, @{const set} converts a list to a set, @{term "xs!n"} returns the 
 \<open>n\<close>-th element of the list \<open>xs\<close> (with 0-indexing), @{term "take n xs"} is the prefix of length \<open>n\<close> 
-of \<open>xs\<close>, and @{term "drop n xs"} is the suffix of \<open>xs\<close> starting at index \<open>n\<close>.\par
+of \<open>xs\<close>, and @{term "drop n xs"} is the suffix of \<open>xs\<close> starting at index \<open>n\<close>.
 
 Pattern matching on a term \<open>\<tau>\<close> is done with the keywords \isakeyword{case} and \isakeyword{of}. For 
 patterns \<open>\<pi>\<^sub>1, \<pi>\<^sub>2, \<dots>, \<pi>\<^sub>n\<close> and expressions \<open>e\<^sub>1, e\<^sub>2, \<dots>, e\<^sub>n\<close>, the expression
-
 \begin{quote}
 \isa{\textsf{case}\ \isafree{\isasymtau}\ \textsf{of}} \<open>\<pi>\<^sub>1 \<Rightarrow> e\<^sub>1 | \<pi>\<^sub>2 \<Rightarrow> e\<^sub>2 | \<dots> | \<pi>\<^sub>n \<Rightarrow> e\<^sub>n\<close>
 \end{quote}
-
 returns \<open>e\<^sub>i\<close> if \<open>\<tau>\<close> matches \<open>\<pi>\<^sub>i\<close> and it does not match any \<open>\<pi>\<^sub>j\<close> with \<open>0 < j < i\<close>. If \<open>\<tau>\<close> matches no
 \<open>\<pi>\<^sub>i\<close>, @{const undefined} is returned. It is worth noting that variables introduced in \<open>\<pi>\<^sub>i\<close> are bound
-on \<open>e\<^sub>i\<close>. A simple example on lists returning @{const Nil} if the input is @{const Nil}, and a 
+on \<open>e\<^sub>i\<close>. 
+
+A simple example on lists returning @{const Nil} if the input is @{const Nil}, and a
 singleton list containing the first element otherwise:
 \begin{quote}
 @{term \<open>case xs of [] \<Rightarrow> [] | y # ys \<Rightarrow> [y]\<close>}
 \end{quote}
 
-Finally, if premises \<open>A\<^sub>1, A\<^sub>2, \<dots>, A\<^sub>n\<close> imply conclusion \<open>B\<close>, we write \[ \<open>\<lbrakk>A\<^sub>1; A\<^sub>2; \<dots>; A\<^sub>n\<rbrakk> \<Longrightarrow> B\<close> \]\<close>
+Finally, if premises \<open>A\<^sub>1, A\<^sub>2, \<dots>, A\<^sub>n\<close> imply \<open>B\<close>, we write \mbox{\<open>\<lbrakk>A\<^sub>1; A\<^sub>2; \<dots>; A\<^sub>n\<rbrakk> \<Longrightarrow> B\<close>.}\<close>
 
 subsubsection \<open>Context-Free Grammars\<close>
 
-text \<open>Nipkow et al.\<^cite>\<open>Nipkow\<close> introduce type @{typ "('n, 't) sym"} for context-free grammar 
-\concept{symbols} as a tagged union consisting of nonterminals (@{const Nt}) and terminals (@{const Tm}) 
-of type @{typ 'n} and @{typ 't} respectively:
-
+text \<open>Our formalization works on top of the formalization of context-free grammars by 
+Nipkow et al.~\<^cite>\<open>Nipkow\<close>. In their theories, they introduce type 
+@{typ "('n, 't) sym"} for context-free grammar \concept{symbols} as a tagged union consisting of 
+nonterminals (@{const Nt}) and terminals (@{const Tm}) of type @{typ 'n} and @{typ 't} respectively:
 @{datatype sym}
 
 Besides defining this type for symbols, they also define the following abbreviations:
@@ -83,46 +88,51 @@ Productions & \<open>('n,'t) prod = 'n \<times> ('n,'t) syms\<close>\\
 Sets of productions & \<open>('n,'t) Prods = ('n,'t) prod set\<close>
 \end{tabular}
 \end{quote}
+where we informally write \<open>(A, \<alpha>) :: ('n, 't) prod\<close> as \<open>A \<rightarrow> \<alpha>\<close>. For \mbox{\<open>\<alpha> :: ('n, 't) syms\<close>}, 
+@{term \<open>Nts_syms \<alpha>\<close>} returns the set of all \<open>X :: 'n\<close> such that @{prop \<open>Nt X \<in> set \<alpha>\<close>}. Similarly 
+for \<open>P :: ('n, 't) Prods\<close>, Nipkow et al. define @{term \<open>Nts P\<close>}:
+\begin{equation*}
+@{term \<open>Nts P = (\<Union>(A,\<alpha>)\<in>P. {A} \<union> Nts_syms \<alpha>)\<close>}.
+\end{equation*}
 
-where we informally write \<open>(A, \<alpha>) :: ('n, 't) prod\<close> as \<open>A \<rightarrow> \<alpha>\<close>.\par 
-Lastly, Nipkow et al. also define the datatype for context-free grammars:
-\isakeyword{datatype} \<open>('n, 't) Cfg = Cfg (('n,'t) Prods) 'n\<close> 
-
+They further define the datatype for context-free grammars:
+\begin{equation*}
+\isakeyword{datatype} \<open>('n, 't) Cfg = Cfg (('n,'t) Prods) 'n\<close>.
+\end{equation*}
 @{term "Cfg P S"} denotes a context-free grammar with production set \<open>P\<close> and start symbol \<open>S\<close>. If 
 @{term "G = Cfg P S"}, @{term "Prods G"} refers to \<open>P\<close>, and analogously, @{term "Start G"} refers to 
-\<open>S\<close>.\par
-A derivation step from \<open>\<phi>\<close> to \<open>\<psi>\<close> under production set \<open>P\<close> is notated as \mbox{@{term \<open>P \<turnstile> \<phi> \<Rightarrow> \<psi>\<close>}}.
-More formally, for any nonterminal \<open>A\<close>, and symbols \<open>\<beta>\<close>, \<open>\<alpha>\<close> and \<open>\<gamma>\<close> holds:
-\begin{quote} 
-@{thm derive.intros[of A \<beta> P \<alpha> \<gamma>]}
-\end{quote}
+\<open>S\<close>.
 
-Moreover, we denote the reflexive transitive closure of derivations by \mbox{@{term \<open>P \<turnstile> \<phi> \<Rightarrow>* \<psi>\<close>}}, 
+A derivation step from \<open>\<phi>\<close> to \<open>\<psi>\<close> under production set \<open>P\<close> is notated as \mbox{@{term \<open>P \<turnstile> \<phi> \<Rightarrow> \<psi>\<close>}}.
+More formally, for \<open>A :: 'n\<close> and \<open>\<alpha>, \<beta>, \<gamma> :: ('n, 't) syms\<close> they define:
+\begin{equation*} 
+@{thm derive.intros[of A \<beta> P \<alpha> \<gamma>]}.
+\end{equation*}
+Moreover, they denote the reflexive transitive closure of derivations by \mbox{@{term \<open>P \<turnstile> \<phi> \<Rightarrow>* \<psi>\<close>}}, 
 and derivations of length \<open>n\<close> by @{term \<open>P \<turnstile> \<phi> \<Rightarrow>(n) \<psi>\<close>}. Rightmost derivations are notated analogously, 
 with \<open>\<Rightarrow>r\<close>, \<open>\<Rightarrow>r*\<close> and \<open>\<Rightarrow>r(n)\<close> respectively.\par
 
-Lastly, Nipkow et al. define the language of a nonterminal w.r.t a set of 
-productions:
-\begin{quote}
-@{thm Lang_def}
-\end{quote}
-And based on this, the language of a grammar:
-\begin{quote}
-\<open>LangS G = Lang (Prods G) (Start G)\<close>
-\end{quote}
+Lastly, Nipkow et al. define the language of a nonterminal w.r.t a set of productions
+\begin{equation*}
+@{thm Lang_def},
+\end{equation*}
+and based on this, the language of a grammar
+\begin{equation*}
+@{term \<open>LangS G\<close>} = @{term [show_abbrevs=false] \<open>Lang (Prods G) (Start G)\<close>}
+\end{equation*}
  
 Besides type variables @{typ 'n} for nonterminals and @{typ 't} for terminals, we use the following 
 variable conventions: for brevity, we refer to \<open>('n, 't) sym\<close> and \<open>('n, 't) syms\<close> simply as @{type sym}
 and @{type syms} respectively; \<open>A, B, C :: 'n\<close>; \<open>a, b, c :: 't\<close>; \<open>u, v, w :: 't list\<close>; and finally
 \<open>\<alpha>, \<beta>, \<gamma> :: ('n, 't) syms\<close>.\par
 
-For further definitions and notation, we defer to the AFP entry by Nipkow et al~\<^cite>\<open>Nipkow\<close>.
-\<close>
+For further definitions and notation, we defer to the AFP entry by Nipkow et al~\<^cite>\<open>Nipkow\<close>.\<close>
 
 section \<open>Previous Work\<close>
 
 section \<open>Basic Definitions\<close>
 subsection \<open>Extended Grammars\<close>
+subsubsection \<open>Reduced Grammars\<close>
 
 text \<open>In general, context-free grammars (CFGs) can contain problematic nonterminals which can be 
 removed from the grammar without altering the language. Working with grammars that lack such 
@@ -130,61 +140,72 @@ nonterminals is ideal, since having them increases computational complexity and 
 less well-behaved.
 
 \begin{example}
-Let \<open>G\<close> be a CFG with productions:
+Let \<open>G\<close> be a CFG with @{term \<open>S = Start G\<close>} and productions:
 \begin{center}
 \begin{tabular}{cc}
-\<open>Start G \<rightarrow> A | AB\<close> & \<open>A \<rightarrow> aA | a\<close>\\
+\<open>S \<rightarrow> A | AB\<close> & \<open>A \<rightarrow> aA | a\<close>\\
 \<open>C \<rightarrow> ac | BCD\<close> & \<open>D \<rightarrow> BC | D\<close>
 \end{tabular}
 \end{center}
-
-Each nonterminal except for \<open>Start G\<close> and \<open>A\<close> carries problems with it:
+Each nonterminal except for \<open>S\<close> and \<open>A\<close> carries problems with it:
 \begin{itemize}
-\item There are no productions where \<open>B\<close> is on the left-hand side. This means that if \<open>Start G\<close> 
+\item There are no productions where \<open>B\<close> is on the left-hand side. This means that if \<open>S\<close> 
 reaches a sentential form \<open>\<alpha>\<close> such that \<open>Nt B \<in> set \<alpha>\<close>, no word will be derived from \<open>\<alpha>\<close>. 
-\item \<open>Start G\<close> cannot reach \<open>C\<close>, meaning no productions containing \<open>C\<close>, or reachable only 
+\item \<open>S\<close> cannot reach \<open>C\<close>, meaning no productions containing \<open>C\<close>, or reachable only 
 through \<open>C\<close> (e.g. reaching \<open>D\<close> using production \mbox{\<open>C \<rightarrow> BCD\<close>}), can be used to derive words in \<open>LangS G\<close>.
 \item \<open>D\<close>, as opposed to \<open>B\<close>, does show up on the LHS of certain productions, but none of these productions
 can lead to a word: \<open>D \<rightarrow> BC\<close> contains \<open>B\<close>, which cannot derive a \<open>'t list\<close>, and \<open>D \<rightarrow> D\<close> has no effect.
-Furthermore, similarly to \<open>C\<close>, \<open>D\<close> cannot be reached by \<open>Start G\<close>.
+Furthermore, similarly to \<open>C\<close>, \<open>D\<close> cannot be reached by \<open>S\<close>.
 \end{itemize}
 \end{example}
 
-Nipkow et al.\<^cite>\<open>Nipkow\<close> define \concept{useful} nonterminals w.r.t. a set of productions and a start 
+Nipkow et al. define \concept{useful} nonterminals w.r.t. a set of productions and a start 
 symbol:
-\begin{quote}
-@{abbrev productives}\\
-@{thm useful_def}
-\end{quote}
-
+\begin{gather*}
+@{abbrev \<open>productives P \<alpha>\<close>}\\
+\begin{multlined}
+\<open>useful P S A =\<close>\ (@{term \<open>\<exists>\<beta>. P \<turnstile> [Nt S] \<Rightarrow>* \<beta>\<close>}\\
+  {} \wedge @{term \<open>Nt A \<in> set \<beta> \<and> productives P \<beta>\<close>})
+\end{multlined}
+\end{gather*}
 For a CFG \<open>G\<close>, \<open>A :: 'n\<close> is \concept{reachable} if there exists a \<open>\<beta> :: syms\<close> such that 
 \mbox{\<open>A \<in> set \<beta>\<close>} and @{prop \<open>Prods G \<turnstile> [Nt (Start G)] \<Rightarrow>* \<beta>\<close>}. Otherwise, it is \concept{unreachable}.
-Similarly, it is \concept{productive} if @{prop \<open>productives (Prods G) [Nt A]\<close>} holds, and 
-\concept{unproductive} otherwise. A useful nonterminal is therefore a nonterminal that is both 
-reachable and productive.\par
+Similarly, it is \concept{productive} if @{prop [source] \<open>productives (Prods G) [Nt A]\<close>} holds, as 
+defined by Nipkow et al. as well:
+\begin{equation*}.
+@{abbrev \<open>productive (Prods G) A\<close>}
+\end{equation*}
+Similarly to reachable terminals, a nonterminal that is not productive is \concept{unproductive}. A 
+useful nonterminal is therefore a nonterminal that is both reachable and productive. 
 
-Nipkow et al. have proved that removing all unreachable and unproductive nonterminals preserves the
-language:
-\begin{quote}
-@{thm restrict_Nts_def}\\
-@{thm Lang_restrict_useful}
-\end{quote}\<close>
+Nipkow et al. have also proved that removing all nonterminals that are unreachable or unproductive, 
+i.e. all non-useful nonterminals, preserves the language~\cite[Lemma Lang\_restrict\_useful]{Nipkow}:
+\begin{lemma}
+Let 
+\[@{term [source] \<open>restrict_Nts R P = {(A,\<alpha>) \<in> P. \<forall>B \<in> {A} \<union> Nts_syms \<alpha>. R B}\<close>}. \]
+Then @{thm Lang_restrict_useful}.\qed
+\end{lemma}
+
+With this, we now define the notion of \concept{reduced grammars}.
+\begin{definition}[Reduced grammar]
+\begin{equation*}
+@{thm reduced_def}.
+\end{equation*}
+\end{definition}
+
+Due to the fact that for any CFG we can construct a reduced grammar with equivalent language,
+we can safely constrain our automata to work exclusively with these more well-behaved grammars 
+without sacrificing generality.\<close>
+
+subsubsection \<open>Extending Grammars by a New Start Symbol\<close>
 
 (*<*)
 context Extended_Cfg 
 begin
 (*>*)
 
-text\<open>Based on these definitions, and thanks to the fact that we can construct a CFG with only useful
-symbols equivalent to an arbitrary CFG, we can use these well-behaved grammars as the foundation
-of our automata in future sections, which we will call \concept{reduced grammars}:
-
-\begin{quote}
-@{thm reduced_def}
-\end{quote}
-
-Let \<open>G\<close> be a fixed CFG whose start symbol is \<open>S\<close>. We assume the following properties:
-
+text\<open>From this point onward in this paper, let \<open>G\<close> be a fixed CFG whose start symbol is \<open>S\<close> with the 
+following properties:
 \begin{itemize}
 \item @{prop \<open>finite (Prods G)\<close>}
 \item @{prop \<open>LangS G \<noteq> {}\<close>}
@@ -193,36 +214,46 @@ Let \<open>G\<close> be a fixed CFG whose start symbol is \<open>S\<close>. We a
 
 We extend \<open>G\<close> by a fresh start symbol \<open>S'\<close> with a single production \<open>(S', [Nt S])\<close>. 
 The resulting grammar, which we define to be \<open>G'\<close>, is the \concept{extended grammar}, or the 
-\concept{extension}, of $G$. We analogously refer to the set of productions of $G'$, 
-as the extension of \<open>Prods G\<close> or the \concept{extended set of productions} of $G$. Formally:
-\begin{quote}
+\concept{extension}, of \<open>G\<close>. We analogously refer to \<open>Prods G'\<close> as the extension of \<open>Prods G\<close> or the 
+\concept{extended set of productions} of \<open>G\<close>. Formally:
+\begin{gather*}
 @{thm S'_def}\\
 @{thm G'_def}
-\end{quote}
+\end{gather*}
 
 We now prove that extending a grammar preserves both language and reduction.\<close>
 
 (*<*)
 end
 (*>*)
-
+(* Needed? (trivial?) *)
 text\<open>\begin{lemma}\label{S_deriven_Suc_imp_all_nts_in_Nts}
-Let \<open>G\<close> be an arbitrary CFG. If \mbox{@{prop \<open>Prods G \<turnstile> [Nt (Start G)] \<Rightarrow>(Suc n) \<alpha>\<close>}} and 
-@{prop \<open>A \<in> Nts_syms \<alpha>\<close>}, then @{prop \<open>A \<in> Nts (Prods G)\<close>}.
+If \<open>G\<close> is an arbitrary CFG and there exist \<open>\<alpha> :: syms\<close>, \<open>A :: 'n\<close> where @{prop \<open>A \<in> Nts_syms \<alpha>\<close>} 
+and
+\[ @{prop \<open>Prods G \<turnstile> [Nt (Start G)] \<Rightarrow>(Suc n) \<alpha>\<close>}, \]
+Then @{prop \<open>A \<in> Nts (Prods G)\<close>}.
 \begin{proof}
 We do a proof by induction on \<open>n\<close> for arbitrary \<open>\<alpha>\<close>. In the base case, the derivation is a 
-single step @{prop \<open>Prods G \<turnstile> [Nt (Start G)] \<Rightarrow> \<alpha>\<close>}, meaning \<open>(Start G, \<alpha>) \<in> Prods G\<close>. Together with 
-the fact that \<open>A \<in> Nts_syms \<alpha>\<close>, this implies @{prop \<open>A \<in> Nts (Prods G)\<close>}.\par
-For the inductive case, we must prove the statement holds for \<open>\<alpha>\<close> assuming 
+single step @{prop \<open>Prods G \<turnstile> [Nt (Start G)] \<Rightarrow> \<alpha>\<close>}, meaning \mbox{\<open>(Start G, \<alpha>) \<in> Prods G\<close>}. 
+Together with the fact that \<open>A \<in> Nts_syms \<alpha>\<close>, this implies @{prop \<open>A \<in> Nts (Prods G)\<close>}.
+
+For the inductive step, we must prove the statement holds for \<open>\<alpha>\<close> assuming 
 @{prop \<open>Prods G \<turnstile> [Nt (Start G)] \<Rightarrow>(Suc (Suc n)) \<alpha>\<close>} for some \<open>n\<close> and @{prop \<open>A \<in> Nts_syms \<alpha>\<close>}. 
-This implies there is a last step of the form\par
+This implies there is a last step of the form
+\begin{equation*}
+\<open>Prods G \<turnstile> [Nt (Start G)] \<Rightarrow>(Suc n) \<gamma> @ [Nt B] @ \<delta> \<Rightarrow> \<gamma> @ \<beta> @ \<delta> = \<alpha>\<close>
+\end{equation*}
+with @{term \<open>(B, \<beta>) \<in> Prods G\<close>}. 
 
-\<open>Prods G \<turnstile> [Nt (Start G)] \<Rightarrow>(Suc n) \<gamma> @ [Nt B] @ \<delta> \<Rightarrow> \<gamma> @ \<beta> @ \<delta> = \<alpha>\<close> with \<open>(B, \<beta>) \<in> Prods G\<close>.\par
+We now make a case distinction on whether \<open>A \<in> Nts_syms \<beta>\<close> holds:
 
-We now make a case distinction on whether \<open>A \<in> Nts_syms \<beta>\<close> holds.\\
-If \<open>A \<in> Nts_syms \<beta>\<close>, then \<open>A \<in> Nts (Prods G)\<close> by the fact that \<open>(B, \<beta>) \<in> Prods G\<close> directly.\\
-If \<open>A \<notin> Nts_syms \<beta>\<close>, this together with \<open>A \<in> Nts_syms \<alpha>\<close> implies \<open>A \<in> Nts_syms (\<gamma> @ [Nt B] @ \<delta>)\<close>. 
-By the induction hypothesis, this implies \<open>A \<in> Nts (Prods G)\<close>, and the proof is thus complete.
+If \<open>A \<in> Nts_syms \<beta>\<close>, then \<open>A \<in> Nts (Prods G)\<close> follows directly by the fact that 
+\mbox{\<open>(B, \<beta>) \<in> Prods G\<close>}.
+
+If \<open>A \<notin> Nts_syms \<beta>\<close>, this and \<open>A \<in> Nts_syms \<alpha>\<close> imply
+\[ \<open>A \<in> Nts_syms (\<gamma> @ [Nt B] @ \<delta>)\<close>. \] 
+By the induction hypothesis, this in turn implies \<open>A \<in> Nts (Prods G)\<close>, and the proof is thus 
+complete.
 \end{proof}
 \end{lemma}\<close>
 
@@ -254,24 +285,23 @@ Lemma~\ref{G'_derive_imp_G_derive_if_no_S'} in conjunction with the fact that
 @{thm Lang_preserved}
 \begin{proof} 
 Let @{prop \<open>w \<in> LangS G'\<close>}. Then there exists a derivation of the form
-\begin{equation}\notag
-\<open>Prods G' \<turnstile> [Nt S'] \<Rightarrow> [Nt S] \<Rightarrow>* map Tm w\<close>
-\end{equation}
+\begin{equation*}
+\<open>Prods G' \<turnstile> [Nt S'] \<Rightarrow> [Nt S] \<Rightarrow>* map Tm w\<close>.
+\end{equation*}
 Therefore, there exists an \<open>n :: nat\<close> such that 
-\begin{equation}\notag
+\begin{equation*}
 @{prop \<open>Prods G' \<turnstile> [Nt S'] \<Rightarrow>(Suc n) map Tm w\<close>}.
-\end{equation}
-By Lemma~\ref{G'_deriven_Suc_imp_G_deriven}, this implies the existence of a derivation\\
-@{prop \<open>Prods G \<turnstile> [Nt S] \<Rightarrow>(n) map Tm w\<close>}, and thus @{prop \<open>w \<in> LangS G\<close>}. \\
+\end{equation*}
+By Lemma~\ref{G'_deriven_Suc_imp_G_deriven}, this implies the existence of a derivation
+\mbox{@{prop \<open>Prods G \<turnstile> [Nt S] \<Rightarrow>(n) map Tm w\<close>}}, and thus \mbox{@{prop \<open>w \<in> LangS G\<close>}}.
+
 Conversely, let @{prop \<open>w \<in> LangS G\<close>}. Then there exists a derivation\\
 @{prop \<open>Prods G \<turnstile> [Nt S] \<Rightarrow>* map Tm w\<close>}. Since @{prop \<open>Prods G' \<turnstile> [Nt S'] \<Rightarrow> [Nt S]\<close>} and 
 @{prop \<open>Prods G \<subseteq> Prods G'\<close>}, @{prop \<open>Prods G' \<turnstile> [Nt S'] \<Rightarrow>* map Tm w\<close>} also holds by 
-transitivity and the monotonicity of \<open>\<Rightarrow>*\<close>, as proven by Nipkow et al.:
-
+transitivity and the monotonicity of \<open>\<Rightarrow>*\<close>, as proven by Nipkow et al.~\cite[Lemma derives\_mono]{Nipkow}:
 \begin{quote}
 @{thm derives_mono}
 \end{quote}
-
 Therefore, @{prop \<open>w \<in> LangS G'\<close>}. This completes the proof.
 \end{proof}
 \end{theorem}
@@ -281,9 +311,9 @@ If \<open>G\<close> is reduced and @{prop \<open>LangS G \<noteq> {}\<close>}, \
 \begin{proof}
 Since \<open>G\<close> is reduced, all nonterminals in \<open>Prods G\<close> are useful, and the fact that @{prop \<open>LangS G \<noteq> {}\<close>}
 implies that there exist \<open>\<alpha> :: syms\<close> and \<open>w \<in> LangS G\<close> such that  
-\begin{equation}\notag
-\<open>Prods G \<turnstile> [Nt S] \<Rightarrow> \<alpha> \<Rightarrow>* map Tm w\<close>
-\end{equation}
+\begin{equation*}
+\<open>Prods G \<turnstile> [Nt S] \<Rightarrow> \<alpha> \<Rightarrow>* map Tm w\<close>.
+\end{equation*}
 This implies that \<open>S \<in> Nts (Prods G)\<close>. Since \<open>Prods G \<subseteq> Prods G'\<close>, this
 means that all nonterminals in \<open>Nts (Prods G)\<close> are useful in \<open>Prods G'\<close>. Therefore, to show that 
 \<open>G'\<close> is reduced, it suffices to show that \<open>S'\<close> is useful in \<open>Prods G'\<close>, i.e., reachable and productive. 
@@ -312,34 +342,30 @@ work towards deriving a string, the symbols to the right of the bullet (e.g. \<o
 @{term \<open>[A \<rightarrow> \<alpha> \<cdot> \<beta>]\<close>}) are shifted towards the left. If \<open>(A, \<alpha>@\<beta>) \<in> Prods G\<close>, the item
 @{term \<open>[A \<rightarrow> \<alpha> \<cdot> \<beta>]\<close>} denotes the situation where a word has already been derived from the substring 
 \<open>\<alpha>\<close>, with a suffix still left to be derived from \<open>\<beta>\<close>. We call the symbols that have already been 
-shifted the \concept{history} of the item.\\
+shifted the \concept{history} of the item.
 
 For @{term \<open>[A \<rightarrow> \<alpha> \<cdot> \<beta>]\<close>}, \<open>\<alpha> = \<epsilon>\<close> denotes the situation where nothing has been 
 derived from \<open>A\<close> yet. Analogously, \<open>\<beta> = \<epsilon>\<close> denotes the situation where a substring of the 
 input has been completely derived from \<open>A\<close>. These items are therefore called \concept{initial} and 
 \concept{complete} items respectively. For both of these kinds of item, we write \<open>\<epsilon>\<close> implicitly, 
-e.g., instead of @{term \<open>[A \<rightarrow> \<alpha> \<cdot> \<epsilon>]\<close>}, we write @{term \<open>[A \<rightarrow> \<alpha> \<cdot> ]\<close>}.\par
-
-Additionally, we denote the set of all complete items in a set of items \<open>I\<close> by @{term \<open>completes I\<close>}:
-\begin{quote}
-@{thm completes_def}
-\end{quote}
-
+e.g., instead of @{term \<open>[A \<rightarrow> \<alpha> \<cdot> \<epsilon>]\<close>}, we write @{term \<open>[A \<rightarrow> \<alpha> \<cdot> ]\<close>}. Additionally, we denote the 
+set of all complete items in a set of items \<open>I\<close> by @{term \<open>completes I\<close>}:
+\begin{equation*}
+@{thm completes_def}.
+\end{equation*}
 An item that is not complete is referred to as \concept{noncomplete}, and we correspondingly define
 @{const noncompletes} as the complement of @{const completes}:
-\begin{quote}
-@{abbrev noncompletes}
-\end{quote}
-
+\begin{equation*}
+@{abbrev \<open>noncompletes I\<close>}.
+\end{equation*}
 We also lift the definition of history from items to lists of items:
-\begin{quote}
-@{thm hist_def}
-\end{quote}
-
-Lastly, we refer to the set of all items of a CFG \<open>G\<close> as @{term \<open>It G\<close>}:
-\begin{quote}
-@{thm It_def}
-\end{quote}
+\begin{equation*}
+@{thm hist_def},
+\end{equation*}
+and lastly, we refer to the set of all items of a CFG \<open>G\<close> as @{term \<open>It G\<close>}:
+\begin{equation*}
+@{thm It_def}.
+\end{equation*}
 
 \begin{lemma}\label{in_Prods_iff_in_It}
 @{term \<open>(A, \<alpha>@\<beta>) \<in> Prods G \<longleftrightarrow> [A \<rightarrow> \<alpha> \<cdot> \<beta>] \<in> It G\<close>}
@@ -361,9 +387,7 @@ If \<open>G\<close> is a CFG such that \<open>Prods G\<close> is finite, @{term 
 \begin{proof}
 The definition of @{term \<open>It G\<close>} is clearly equivalent to the union of the sets of items for 
 each production in \<open>Prods G\<close>. Formally:
-
-@{term [display] \<open>It G = (\<Union>(A,w)\<in>Prods G. {[A \<rightarrow> \<alpha> \<cdot> \<beta>] | \<alpha> \<beta>. \<alpha>@\<beta> = w})\<close>}
-
+\[ @{term \<open>It G = (\<Union>(A,w)\<in>Prods G. {[A \<rightarrow> \<alpha> \<cdot> \<beta>] | \<alpha> \<beta>. \<alpha>@\<beta> = w})\<close>}. \]
 By Lemma~\ref{prod_items_finite}, each of these sets is finite, meaning their union is also finite.
 \end{proof}
 \end{lemma}\<close>
@@ -380,8 +404,8 @@ text \<open>Throughout this paper, we define several automata to lay the foundat
 LR(0) parser. Most of these automata, including the parser itself, require a stack to operate, but 
 unlike conventional pushdown automata, it is sometimes necessary for them to read multiple stack 
 symbols in a single transition steps.
-
-We define generalized pushdown automata (GPDAs) as a record of type @{typ "('q, 'a) gpda"} where 
+\begin{definition}[Generalized pushdown automata]
+A generalized pushdown automata (GPDAs) is a record of type @{typ "('q, 'a) gpda"} where 
 @{typ 'q} is the type of stack symbols, @{typ 'a} the type of alphabet symbols, and
 \begin{itemize}
 \item \<open>states :: 'q set\<close> is a finite set of states.
@@ -390,6 +414,7 @@ We define generalized pushdown automata (GPDAs) as a record of type @{typ "('q, 
 \item \<open>nxt :: ('q list \<times> 'a \<times> 'q list) set\<close> is the transition relation consuming input symbols.
 \item \<open>eps :: ('q list \<times> 'q list) set\<close> is the transition relation for \<open>\<epsilon>\<close>-transitions.
 \end{itemize}
+\end{definition}
 
 It is worth noting that, differently from traditional PDAs, GPDAs do not have a dedicated state. 
 Instead, the topmost stack symbols (with varying length) are used to determine the transition. 
@@ -401,7 +426,7 @@ discuss later.
 For \<open>M :: ('q, 'a) gpda\<close> we define a \concept{configuration} as a tuple 
 \<open>(qs, w) :: 'q list \<times> 'a list\<close> where \<open>qs\<close> denotes the current stack, and \<open>w\<close> the remaining input to 
 be read. In accordance with the Isabelle/HOL list datatype, we define the topmost stack symbol as 
-the leftmost list element, deviating from Wilhelm et al. in this regard.\par
+the leftmost list element, deviating from Wilhelm et al. in this regard.
 
 A configuration of \<open>M\<close> is \concept{initial} if the stack consists of a singleton list containing 
 the initial state @{term \<open>init M\<close>}, while a \concept{final} configuration for \<open>M\<close> consists of a 
@@ -409,11 +434,9 @@ singleton list with some final state on the stack after completely consuming the
 i.e., a configuration of the form \<open>([f], \<epsilon>)\<close> for some \<open>f \<in> final M\<close>.
 
 We now define the step relation \<open>\<turnstile>\<close> for GPDAs:
-
 @{thm [display] step_nxt step_eps}
-
 We refer to sequences of configurations as \concept{computations}, and denote \<open>n\<close>-step computations
-with \<open>\<turnstile>(n)\<close>, and its reflexive-transitive closure with \<open>\<turnstile>*\<close>.\par
+with \<open>\<turnstile>(n)\<close>, and its reflexive-transitive closure with \<open>\<turnstile>*\<close>.
 
 \begin{lemma}\label{reachable_imp_substring}
 If @{prop \<open>(ps, w) \<turnstile>* (qs, v)\<close>}, \<open>v\<close> is a suffix of \<open>w\<close>, i.e., there exists a \<open>u\<close> such that 
@@ -426,9 +449,9 @@ step of the computation is a \<open>nxt\<close>-step or an \<open>eps\<close>-st
 
 Finally, we define the \concept{language} @{term \<open>Lang\<close>} for \<open>M\<close> as the set of words for which \<open>M\<close> 
 can reach a final configuration from the corresponding initial configuration:
-\begin{quote}
-@{thm Lang_def}
-\end{quote}\<close>
+\begin{equation*}
+@{thm Lang_def}.
+\end{equation*}\<close>
 
 section \<open>The Item Pushdown Automaton\<close>
 
@@ -451,81 +474,89 @@ abbreviation ipda_stepn :: "('n,'t) item list \<times> 't list \<Rightarrow> nat
 
 (*>*)
 
+subsection \<open>Definition\<close>
+
 text \<open>One of the main objectives in the construction of our parser is determinism. Despite the ability of
 PDAs of recognizing CFLs, they are non-deterministic in general, which means they are not easily
 implemented in practice. In this section, we define the Item Pushdown Automaton to a 
 context-free grammar, from which we will later derive a deterministic parser.\par
 
+\begin{definition}[Item pushdown automaton]
 The \concept{item pushdown automaton} (IPDA) to a CFG \<open>G\<close> with extension \<open>G'\<close> is the 
-\<open>(('n, 't) item, 't) gpda\<close>:
-\begin{quote}
-@{term \<open>I\<^sub>G = \<lparr>gpda.states = It G', init = [S' \<rightarrow> \<cdot> [Nt S]], final = {mbox [S' \<rightarrow> [Nt S] \<cdot> ]}, 
-  nxt = \<Delta>, eps = \<E>\<rparr>\<close>}
-\end{quote}
-
-Overall, the IPDA has three types of transitions. We call transitions in @{const nxt} \concept{shifting} 
-transitions:
-
-\begin{multline}
-\<open>\<Delta> = {([[X \<rightarrow> \<beta> \<cdot> Tm a # \<gamma>]], a, [[X \<rightarrow> \<beta> @ [Tm a] \<cdot> \<gamma>]])\<close> \\
-\<open>|X \<beta> a \<gamma>. (X, \<beta> @ Tm a # \<gamma>) \<in> Prods G'}\<close>
-\end{multline}
-
-The other two transition types are in \<open>eps\<close>; we have
-\begin{itemize}
-\item \concept{expanding} transitions\\ 
-\begin{multline}
+\mbox{\<open>(('n, 't) item, 't) gpda\<close>}:
+\begin{multline*}
+  \<open>I\<^sub>G = \<lparr>gpda.states = It G', init = [S' \<rightarrow> \<cdot> [Nt S]],\<close>\\
+  \<open>final = {[S' \<rightarrow> [Nt S] \<cdot> ]}, nxt = \<Delta>, eps = \<E>\<rparr>\<close>
+\end{multline*}
+where 
+\begin{multline*}
+\<open>\<Delta> = {([[X \<rightarrow> \<beta> \<cdot> Tm a # \<gamma>]], a, [[X \<rightarrow> \<beta> @ [Tm a] \<cdot> \<gamma>]])\<close>\\
+\<open>| X \<beta> a \<gamma>. (X, \<beta> @ Tm a # \<gamma>) \<in> Prods G'}\<close>
+\end{multline*}
+and \<open>\<E> = E \<union> R\<close> for
+\begin{gather*}
+\begin{multlined}
   \<open>E = {([[X \<rightarrow> \<beta> \<cdot> Nt Y # \<gamma>]], [[Y \<rightarrow> \<cdot> \<alpha>], [X \<rightarrow> \<beta> \<cdot> Nt Y # \<gamma>]])\<close>\\ 
-  \<open>| X \<beta> Y \<gamma> \<alpha>. (X, \<beta> @ Nt Y # \<gamma>) \<in> Prods G' \<and> (Y, \<alpha>) \<in> Prods G'}\<close> \mathrm{,\ and}
-\end{multline}
-\item \concept{reducing} transitions\\
-\begin{multline}
+  \<open>| X \<beta> Y \<gamma> \<alpha>. (X, \<beta> @ Nt Y # \<gamma>) \<in> Prods G' \<and> (Y, \<alpha>) \<in> Prods G'}\<close>
+\end{multlined}\\
+\begin{multlined}
   \<open>R = {([[Y \<rightarrow> \<alpha> \<cdot> ], [X \<rightarrow> \<beta> \<cdot> Nt Y # \<gamma>]], [[X \<rightarrow> \<beta> @ [Nt Y] \<cdot> \<gamma>]])\<close>\\
   \<open>| Y \<alpha> X \<beta> \<gamma>. (X, \<beta> @ Nt Y # \<gamma>) \<in> Prods G' \<and> (Y, \<alpha>) \<in> Prods G'}\<close>
-\end{multline}
-\end{itemize}
+\end{multlined}
+\end{gather*}
+\end{definition}
 
-We then define \<open>\<E> = E \<union> R\<close>. Our definitions differ slightly from those by Wilhelm et al.: in all
+Overall, the IPDA has three types of transitions. We call transitions in @{const nxt} \concept{shifting} 
+transitions, transitions in @{term \<open>E \<subseteq> \<E>\<close>} \concept{expanding} transitions, and transitions in 
+@{term \<open>R \<subseteq> \<E>\<close>} \concept{reducing} transitions.
+
+Our definitions differ slightly from those by Wilhelm et al.: in all
 transition sets, we explicitly restrict the elements to items that correspond to productions of \<open>G'\<close>.
 In their book, Wilhelm et al. define the transition relation of a GPDA with state set \<open>Q\<close> and input
-alphabet \<open>V\<^sub>T\<close> to be a subset of \<open>Q\<^sup>+ \<times> V\<^sub>T \<times> Q\<^sup>*\<close>. We approximate this in the record type of GPDAs, 
+alphabet \<open>V\<^sub>T\<close> to be a subset of \mbox{\<open>Q\<^sup>+ \<times> V\<^sub>T \<times> Q\<^sup>*\<close>}. We approximate this in the record type of GPDAs, 
 as we stated before, by definining \mbox{\<open>nxt :: ('q list \<times> 'a \<times> 'q list) set\<close>} and 
-\<open>eps :: ('q list \<times> 'q list) set\<close> for a \<open>('q, 'a) gpda\<close>. Our definitions of \mbox{\<open>nxt IPDA\<close>} and \<open>eps IPDA\<close>
+\mbox{\<open>eps :: ('q list \<times> 'q list) set\<close>} for a \<open>('q, 'a) gpda\<close>. Our definitions of \mbox{\<open>nxt IPDA\<close>} and \<open>eps IPDA\<close>
 therefore enforce this by explicitly restricting the set to items whose corresponding production is 
 in \<open>Prods G'\<close>, which is equivalent to the items themselves being in @{term \<open>It G'\<close>} by 
 Lemma~\ref{in_Prods_iff_in_It}.
 
-%\begin{lemma
+%\begin{lemma}
 %\<open>I\<^sub>G\<close> fullfills all GPDA assumptions
 %\begin{proof}
-%We begin by proving the 
+%\end{proof} 
 %\end{lemma}
 
 Intuitively, \<open>I\<^sub>G\<close> accepts a word \<open>w\<close> by finding a rightmost derivation 
-@{term \<open>Prods G' \<turnstile> [Nt S'] \<Rightarrow>r* map Tm w\<close>}:\par
-If the current topmost stack item is @{term \<open>[A \<rightarrow> \<alpha> \<cdot> Tm a # \<beta>]\<close>} for any \<open>a :: 't\<close>, \<open>I\<^sub>G\<close> will 
-invariably shift \<open>Tm a\<close>, effectively replacing this topmost item by @{term \<open>[A \<rightarrow> \<alpha> @ [Tm a] \<cdot> \<beta>]\<close>}. 
+\[ @{term \<open>Prods G' \<turnstile> [Nt S'] \<Rightarrow>r* map Tm w\<close>}. \]
+If the current topmost stack item is @{term \<open>[A \<rightarrow> \<alpha> \<cdot> Tm a # \<beta>]\<close>} for any \mbox{\<open>a :: 't\<close>}, \<open>I\<^sub>G\<close> will 
+invariably shift \<open>Tm a\<close>, effectively replacing this topmost item by @{term \<open>mbox [A \<rightarrow> \<alpha> @ [Tm a] \<cdot> \<beta>]\<close>}. 
 Similarly, if the topmost item is some complete item @{term \<open>[Y \<rightarrow> \<alpha> \<cdot> ]\<close>}, it will reduce the item 
 and shift \<open>Nt Y\<close> on the second-topmost item if possible. If the stack is 
 @{term \<open>[Y \<rightarrow> \<alpha> \<cdot> ] # [X \<rightarrow> \<beta> \<cdot> Nt Y # \<gamma>] # \<rho>\<close>}, the act of reducing the first two items to 
-@{term \<open>[X \<rightarrow> \<beta> @ [Nt Y] \<cdot> \<gamma>]\<close>} is equivalent to the backwards (i.e. from right to left)
-application of the rightmost derivation step:
+@{term \<open>[X \<rightarrow> \<beta> @ [Nt Y] \<cdot> \<gamma>]\<close>} is equivalent to the backwards (i.e. right-to-left)
+application of a rightmost derivation step for some \<open>u :: 't list\<close> of the form
+\begin{equation*}
+@{prop \<open>Prods G' \<turnstile> \<beta> @ Nt Y # map Tm u \<Rightarrow>r \<beta> @ \<alpha> @ map Tm u\<close>}.
+\end{equation*}
 
-\[ @{prop \<open>Prods G' \<turnstile> \<beta> @ Nt Y # map Tm u \<Rightarrow>r \<beta> @ \<alpha> @ map Tm u\<close>} \mathrm{\ for\ some\ } \<open>u\<close> \]
-
-The most interesting case, however, is the expanding case: this is the only transition type 
-where nondeterministic behavior actually presents itself. While reducing transitions correspond to the
-IPDA applying a backward step in a rightmost derivation, the expanding step is essentially the IPDA
-nondeterministically choosing \emph{which} production to reduce: as we will later prove, if the IPDA
-expands 
-\[ @{term \<open>[X \<rightarrow> \<beta> \<cdot> Nt Y # \<gamma>] # \<rho>\<close>} \] 
-to \mbox{@{term \<open>[Y \<rightarrow> \<cdot> \<alpha> ] # [X \<rightarrow> \<beta> \<cdot> Nt Y # \<gamma>] # \<rho>\<close>}}, 
-it will only complete \<open>\<alpha>\<close>, i.e., reach @{term \<open>[Y \<rightarrow> \<alpha> \<cdot> ] # [X \<rightarrow> \<beta> \<cdot> Nt Y # \<gamma>] # \<rho>\<close>}, if for some 
-prefix \<open>u\<close> of the remaining input word \<open>w = uv\<close>, @{prop \<open>Prods G' \<turnstile> \<alpha> \<Rightarrow>* map Tm u\<close>} holds.
+Lastly, the expanding case is the only transition type where nondeterministic behavior actually 
+presents itself. While reducing transitions correspond to the IPDA applying a backward step in a 
+rightmost derivation, the expanding step is essentially the IPDA nondeterministically choosing 
+\emph{which} production to reduce: as we will later prove, if the IPDA performs the expansion
+\begin{multline*}
+@{term \<open>([X \<rightarrow> \<beta> \<cdot> Nt Y # \<gamma>] # \<rho>, w)\<close>}\\
+  \<open>\<turnstile>\<close>\ @{term \<open>([Y \<rightarrow> \<cdot> \<alpha> ] # [X \<rightarrow> \<beta> \<cdot> Nt Y # \<gamma>] # \<rho>, w)\<close>}
+\end{multline*}
+it will only complete \<open>\<alpha>\<close>, i.e., reach a configuration with stack 
+\[ @{term \<open>[Y \<rightarrow> \<alpha> \<cdot> ] # [X \<rightarrow> \<beta> \<cdot> Nt Y # \<gamma>] # \<rho>\<close>} \]
+if for some prefix \<open>u\<close> of the remaining input word \<open>w = uv\<close> holds 
+\[ @{prop \<open>Prods G' \<turnstile> \<alpha> \<Rightarrow>* map Tm u\<close>}. \]
  
-We will now work towards proving that \<open>I\<^sub>G\<close> accepts exactly \<open>LangS G\<close>.
+We will now work towards proving that \<open>I\<^sub>G\<close> accepts exactly @{term \<open>LangS G\<close>}.\<close>
 
-\begin{lemma}\label{reducing_imp_in_Prods_G}
+subsection \<open>Language Equivalence\<close>
+
+text\<open>\begin{lemma}\label{reducing_imp_in_Prods_G}
 @{thm reducing_imp_in_Prods_G}
 \begin{proof}
 Because \<open>I\<^sub>G\<close> transitions are only defined for elements of @{term \<open>It G\<close>}, we know that 
@@ -537,9 +568,10 @@ we know no such production exists, this would be a contradiction. Therefore, \<o
 
 \begin{corollary}\label{steps_shift_decomp}
 If there exists a computation of the form  
-\begin{quote}
-\<open>(\<rho>, u @ v) \<turnstile>* ([A \<rightarrow> \<alpha> \<cdot> Tm a # \<beta>] # \<sigma>, a # v) \<turnstile> (\<tau>, v)\<close>,
-\end{quote}
+\begin{equation*}
+@{term \<open>(\<rho>, u @ v) \<turnstile>* ([A \<rightarrow> \<alpha> \<cdot> Tm a # \<beta>] # \<sigma>, a # v)\<close>} 
+  \vdash @{term (rhs) \<open>([A \<rightarrow> \<alpha> \<cdot> Tm a # \<beta>] # \<sigma>, a # v) \<turnstile> (\<tau>, v)\<close>},
+\end{equation*}
 then there exists an \<open>x :: 't list\<close> such that \<open>u = xa\<close>.
 \begin{proof}
 This is a direct consequence of Lemma~\ref{reachable_imp_substring}.
@@ -550,73 +582,69 @@ This is a direct consequence of Lemma~\ref{reachable_imp_substring}.
 @{prop \<open>([init M], u @ v) \<turnstile>* (rev \<rho>, v)\<close>} implies\\ @{prop \<open>Prods G \<turnstile> hist \<rho> \<Rightarrow>* map Tm u\<close>}.
 \begin{proof}
 We do a proof by induction on the length \<open>n\<close> of the computation for arbitrary \<open>u, v,\<close> and \<open>\<rho>\<close>.\\
-If @{term "([init M], u @ v) \<turnstile>(0) (rev \<rho>, v)"}, then 
-\[ \<open>[init M] = rev \<rho> = [[S' \<rightarrow> \<cdot> [Nt S]]]\<close> \mathrm{\ and \ } @{prop \<open>u @ v = v\<close>} \] 
+If @{term "([init M], u @ v) \<turnstile>(0) (rev \<rho>, v)"}, then
+\begin{gather*} 
+\<open>[init M] = rev \<rho> = [[S' \<rightarrow> \<cdot> [Nt S]]]\<close> \text{ and } @{prop \<open>u @ v = v\<close>} 
+\end{gather*}
 hold. This in turn implies @{prop \<open>hist \<rho> = []\<close>} and @{prop \<open>u = []\<close>}. Since
-\mbox{@{prop \<open>Prods G \<turnstile> [] \<Rightarrow>* []\<close>}} holds, the invariant holds.\par
+\mbox{@{prop \<open>Prods G \<turnstile> [] \<Rightarrow>* []\<close>}} holds, the invariant holds.
 
 On the other hand, if @{term "([init M], u @ v) \<turnstile>(Suc n) (rev \<rho>, v)"} for some \<open>n :: nat\<close>, there 
 exist \<open>\<sigma> :: item list\<close> and \<open>w :: 't list\<close> where
 \begin{equation}\label{eq:ipda.invariant.stepn}
-\<open>([init M], u @ v) \<turnstile>(n) (rev \<sigma>, w) \<turnstile> (rev \<rho>, v)\<close>
+\<open>([init M], u @ v) \<turnstile>(n) (rev \<sigma>, w) \<turnstile> (rev \<rho>, v)\<close>.
 \end{equation}
-We now make a case distinction on the final step of the computation.\par
+We now make a case distinction on the final step of the computation.
 
 If the last step was a shifting transition there exist \<open>A, \<alpha>, a, \<beta>, \<tau>, a, \<close> and \<open>x\<close> such that
-\begin{equation}\label{eq:ipda.invariant.shift}
-@{term \<open>(rev \<sigma>, w) = ([A \<rightarrow> \<alpha> \<cdot> Tm a # \<beta>] # \<tau>, a # v)\<close>}\mathrm{\ and}
-\end{equation}
-\begin{equation}\label{eq:ipda.invariant.rho_shift}
-@{term \<open>rev \<rho> = [A \<rightarrow> \<alpha> @ [Tm a] \<cdot> \<beta>] # \<tau>\<close>}
-\end{equation}
-
+\begin{gather}
+@{term \<open>(rev \<sigma>, w) = ([A \<rightarrow> \<alpha> \<cdot> Tm a # \<beta>] # \<tau>, a # v)\<close>}\label{eq:ipda.invariant.shift}
+\intertext{and}
+@{term \<open>rev \<rho> = [A \<rightarrow> \<alpha> @ [Tm a] \<cdot> \<beta>] # \<tau>\<close>}\label{eq:ipda.invariant.rho_shift}.
+\end{gather}
 With Corollary~\ref{steps_shift_decomp}, this implies the existence of some \<open>y :: 't list\<close> such that
-\mbox{\<open>u = ya\<close>}. This, together with (\ref{eq:ipda.invariant.stepn}), (\ref{eq:ipda.invariant.shift}), and 
-the induction hypothesis implies 
+\mbox{\<open>u = ya\<close>}. This, together with \eqref{eq:ipda.invariant.stepn}, 
+\eqref{eq:ipda.invariant.shift}, and the induction hypothesis implies 
 \begin{equation}\label{eq:ipda.invariant.ih_shift}
-@{prop \<open>Prods G \<turnstile> hist \<sigma> \<Rightarrow>* map Tm y\<close>}
+@{prop \<open>Prods G \<turnstile> hist \<sigma> \<Rightarrow>* map Tm y\<close>}.
 \end{equation}
 
-Furthermore, from (\ref{eq:ipda.invariant.shift}) and (\ref{eq:ipda.invariant.rho_shift}) follows
-\[ \<open>hist \<rho> = hist (rev \<tau>) @ \<alpha> @ [Tm a] = hist \<sigma> @ [Tm a]\<close> \]
-
-This, \<open>u = ya\<close> and (\ref{eq:ipda.invariant.ih_shift}) imply 
-\[ \<open>Prods G \<turnstile> hist \<rho> \<Rightarrow>* ya = u\<close> \]
-This satisfies the invariant.\par
+Furthermore, from \eqref{eq:ipda.invariant.shift} and \eqref{eq:ipda.invariant.rho_shift} follows
+\[ \<open>hist \<rho> = hist (rev \<tau>) @ \<alpha> @ [Tm a] = hist \<sigma> @ [Tm a]\<close>. \]
+This, \<open>u = ya\<close> and \eqref{eq:ipda.invariant.ih_shift} imply 
+\[ \<open>Prods G \<turnstile> hist \<rho> \<Rightarrow>* ya = u\<close>. \]
+This satisfies the invariant.
 
 For the reducing case, we have 
-
-\begin{equation}\label{eq:ipda.invariant.reduce}
-@{term \<open>(rev \<sigma>, w) = ([Y \<rightarrow> \<alpha> \<cdot> ] # [X \<rightarrow> \<beta> \<cdot> Nt Y # \<gamma>] # \<tau>, v)\<close>}\mathrm{\ and}
-\end{equation}
-\begin{equation}\label{eq:ipda.invariant.rho_reduce}
-@{term \<open>rev \<rho> = [X \<rightarrow> \<beta> @ [Nt Y] \<cdot> \<gamma>] # \<tau>\<close>}
-\end{equation}
-
+\begin{gather}
+@{term \<open>(rev \<sigma>, w) = ([Y \<rightarrow> \<alpha> \<cdot> ] # [X \<rightarrow> \<beta> \<cdot> Nt Y # \<gamma>] # \<tau>, v)\<close>}\label{eq:ipda.invariant.reduce}\\
+\intertext{and} @{term \<open>rev \<rho> = [X \<rightarrow> \<beta> @ [Nt Y] \<cdot> \<gamma>] # \<tau>\<close>}\label{eq:ipda.invariant.rho_reduce}
+\end{gather}
 for some \<open>Y, \<alpha>, X, \<beta>, \<gamma>\<close> and \<open>\<tau>\<close>. By Lemma~\ref{reducing_imp_in_Prods_G}, we know that 
-\mbox{@{prop \<open>(Y, \<alpha>) \<in> Prods G\<close>}}. Furthermore, (\ref{eq:ipda.invariant.reduce}) and 
-(\ref{eq:ipda.invariant.rho_reduce}) imply @{prop \<open>hist \<rho> = hist (rev \<tau>) @ \<beta> @ [Nt Y]\<close>} and 
+\mbox{@{prop \<open>(Y, \<alpha>) \<in> Prods G\<close>}}. Furthermore, \eqref{eq:ipda.invariant.reduce} and 
+\eqref{eq:ipda.invariant.rho_reduce} imply @{prop \<open>hist \<rho> = hist (rev \<tau>) @ \<beta> @ [Nt Y]\<close>} and 
 \mbox{@{prop \<open>hist \<sigma> = hist (rev \<tau>) @ \<beta> @ \<alpha>\<close>}}. From this follows
-
 \begin{equation}\label{eq:ipda.invariant.reduce_rs}
-@{prop \<open>Prods G \<turnstile> hist \<rho> \<Rightarrow> hist \<sigma>\<close>}
+@{prop \<open>Prods G \<turnstile> hist \<rho> \<Rightarrow> hist \<sigma>\<close>}.
 \end{equation}
 
-Furthermore, the induction hypothesis along with (\ref{eq:ipda.invariant.stepn}) and 
-(\ref{eq:ipda.invariant.reduce}) implies  
-
-\[ @{prop \<open>Prods G \<turnstile> hist \<sigma> \<Rightarrow>* map Tm u\<close>} \]
-
-Lastly, @{prop \<open>Prods G \<turnstile> hist \<rho> \<Rightarrow>* map Tm u\<close>} follows from this and 
-(\ref{eq:ipda.invariant.reduce_rs}) by transitivity, fulfilling the invariant.
+Furthermore, the induction hypothesis along with \eqref{eq:ipda.invariant.stepn} and 
+\eqref{eq:ipda.invariant.reduce} implies  
+\[ @{prop \<open>Prods G \<turnstile> hist \<sigma> \<Rightarrow>* map Tm u\<close>}. \]
+@{prop \<open>Prods G \<turnstile> hist \<rho> \<Rightarrow>* map Tm u\<close>} follows from this and \eqref{eq:ipda.invariant.reduce_rs} by 
+transitivity, fulfilling the invariant.
 
 Finally, in the expanding case we have 
-\[ \<open>(rev \<sigma>, w) = ([X \<rightarrow> \<beta> \<cdot> Nt Y # \<gamma>] # \<tau>, v)\<close> \mathrm{\ and} \]
-\[ \<open>rev \<rho> = [Y \<rightarrow> [] \<cdot> \<alpha>] # [X \<rightarrow> \<beta> \<cdot> Nt Y # \<gamma>] # \<tau>\<close> \]
-With the induction hypothesis and (\ref{eq:ipda.invariant.stepn}), this implies
-
-\[ \<open>hist \<rho> = hist \<sigma>\<close> \mathrm{\ and \ }  \<open>Prods G \<turnstile> hist \<sigma> \<Rightarrow>* map Tm u\<close> \]
-
+\begin{gather*}
+\<open>(rev \<sigma>, w) = ([X \<rightarrow> \<beta> \<cdot> Nt Y # \<gamma>] # \<tau>, v)\<close> \intertext{and} 
+  \<open>rev \<rho> = [Y \<rightarrow> [] \<cdot> \<alpha>] # [X \<rightarrow> \<beta> \<cdot> Nt Y # \<gamma>] # \<tau>\<close> 
+\end{gather*}
+With the induction hypothesis and \eqref{eq:ipda.invariant.stepn}, this implies
+\begin{gather*}
+\<open>hist \<rho> = hist \<sigma>\<close>\\ 
+\intertext{and}
+\<open>Prods G \<turnstile> hist \<sigma> \<Rightarrow>* map Tm u\<close>.
+\end{gather*}
 The invariant is therefore satisfied, completing the proof.
 \end{proof}
 \end{lemma}
@@ -625,8 +653,8 @@ The invariant is therefore satisfied, completing the proof.
 @{term \<open>gpda.Lang I\<^sub>G \<subseteq> LangS G\<close>}
 \begin{proof}
 Assume @{prop \<open>w \<in> gpda.Lang I\<^sub>G\<close>}. Then, 
-\[ \<open>([init I\<^sub>G], w) =\<close>\ @{prop \<open>([init I\<^sub>G], w @ [])  \<turnstile>* ([[S' \<rightarrow> [Nt S] \<cdot> ]], [])\<close>} \] By 
-Lemma~\ref{ipda.invariant}, this implies @{prop \<open>Prods G \<turnstile> hist [final_state] \<Rightarrow>* map Tm w\<close>}.
+\[ \<open>([init I\<^sub>G], w) =\<close>\ @{prop \<open>([init I\<^sub>G], w @ [])  \<turnstile>* ([[S' \<rightarrow> [Nt S] \<cdot> ]], [])\<close>}. \] 
+By Lemma~\ref{ipda.invariant}, this implies @{prop \<open>Prods G \<turnstile> hist [final_state] \<Rightarrow>* map Tm w\<close>}.
 Since @{prop \<open>hist [final_state] = [Nt S]\<close>}, this proves that @{prop \<open>w \<in> LangS G\<close>}.  
 \end{proof}
 \end{lemma}
@@ -635,16 +663,17 @@ And now, we prove the other direction:
 
 \begin{lemma}\label{completes_Tms}
 If @{prop \<open>(A, \<alpha> @ map Tm u @ \<beta>) \<in> Prods G' \<close>}, then 
-\[ @{prop \<open>([A \<rightarrow> \<alpha> \<cdot> map Tm u @ \<beta>]#\<rho>, u@v) \<turnstile>* ([A \<rightarrow> \<alpha> @ map Tm u \<cdot> \<beta>]#\<rho>, v)\<close>} \]
+\[ @{prop \<open>([A \<rightarrow> \<alpha> \<cdot> map Tm u @ \<beta>]#\<rho>, u@v) \<turnstile>* ([A \<rightarrow> \<alpha> @ map Tm u \<cdot> \<beta>]#\<rho>, v)\<close>}. \]
 \begin{proof}
 Trivial by induction on the length of \<open>u\<close>.
 \end{proof}
 \end{lemma}
 
 \begin{lemma}\label{derives_imp_completes}[Derivation implies IPDA completion]
-If @{prop \<open>Prods G' \<turnstile> \<beta> \<Rightarrow>* map Tm w\<close>} and @{prop \<open>(A, \<alpha> @ \<beta> @ \<gamma>) \<in> Prods G'\<close>}, then for any 
-\<open>\<rho>, x\<close> holds: 
-\[ @{prop \<open>([A \<rightarrow> \<alpha> \<cdot> \<beta>@\<gamma>] # \<rho>, w @ x) \<turnstile>* ([A \<rightarrow> \<alpha>@\<beta> \<cdot> \<gamma>] # \<rho>, x)\<close>} \]
+If 
+\[ @{prop \<open>Prods G' \<turnstile> \<beta> \<Rightarrow>* map Tm w\<close>} \] 
+and @{prop \<open>(A, \<alpha> @ \<beta> @ \<gamma>) \<in> Prods G'\<close>}, then for any \<open>\<rho>, x\<close> holds: 
+\[ @{prop \<open>([A \<rightarrow> \<alpha> \<cdot> \<beta>@\<gamma>] # \<rho>, w @ x) \<turnstile>* ([A \<rightarrow> \<alpha>@\<beta> \<cdot> \<gamma>] # \<rho>, x)\<close>}. \]
 \begin{proof}
 We do a proof by strong induction on the length of the derivation \<open>n\<close>.\par
 If \<open>n = 0\<close>, \<open>\<beta> = map Tm w\<close>, and the implication holds by Lemma~\ref{completes_Tms}.\par
@@ -654,117 +683,90 @@ If \<open>n = Suc m\<close> for some \<open>m :: nat\<close>, the derivation can
 \begin{gather}
 @{prop \<open>\<beta> = \<delta>\<^sub>1 @ Nt X # \<delta>\<^sub>2\<close>}\label{d_imp_c.b_decomp(1)}\\
 @{prop \<open>w = u @ v @ y\<close>}\label{d_imp_c.b_decomp(2)}\\
-@{prop \<open>Prods G' \<turnstile> \<delta>\<^sub>1 \<Rightarrow>(i) map Tm u\<close>}\\
-@{prop \<open>Prods G' \<turnstile> [Nt X] \<Rightarrow>(j) map Tm v\<close>}\\
-@{prop \<open>Prods G' \<turnstile> \<delta>\<^sub>2 \<Rightarrow>(k) map Tm y\<close>}\\
-@{prop \<open>n = i + j + k\<close>}\label{d_imp_c.b_decomp(6)}
+@{prop \<open>Prods G' \<turnstile> \<delta>\<^sub>1 \<Rightarrow>(i) map Tm u\<close>}\label{d_imp_c.d1}\\
+@{prop \<open>Prods G' \<turnstile> [Nt X] \<Rightarrow>(j) map Tm v\<close>}\label{d_imp_c.X}\\
+@{prop \<open>Prods G' \<turnstile> \<delta>\<^sub>2 \<Rightarrow>(k) map Tm y\<close>}\label{d_imp_c.d2}\\
+@{prop \<open>n = i + j + k\<close>}.\label{d_imp_c.b_decomp(6)}
 \end{gather}
 \end{subequations}
-
 Furthermore, @{prop \<open>Prods G' \<turnstile> [Nt X] \<Rightarrow>(j) map Tm v\<close>} implies @{prop \<open>j > 0\<close>}, since @{prop \<open>j = 0\<close>}
 would imply @{prop \<open>[Nt X] = map Tm v\<close>}, which is a contradiction. We will now do a case distinction 
 on whether @{prop \<open>j = n\<close>} holds.\par
-If \<open>j = n\<close>, then \<open>i = j = 0\<close> and therefore
- 
-\begin{equation}\label{d_imp_c.d1u_d2y}
-\<open>\<delta>\<^sub>1 = map Tm u\<close>\ \mathrm{and\ } \<open>\<delta>\<^sub>2 = map Tm y\<close>
-\end{equation} 
-
-hold. \<open>j = n\<close> also
-implies the existence of some \<open>\<beta>' :: syms\<close> such that 
-
+If \<open>j = n\<close>, then \<open>i = k = 0\<close> and therefore
+\begin{gather}\label{d_imp_c.d1u_d2y}
+\<open>\<delta>\<^sub>1 = map Tm u\<close> \text{ and } \<open>\<delta>\<^sub>2 = map Tm y\<close>
+\end{gather} 
+hold. \<open>j = n\<close> also implies the existence of some \<open>\<beta>' :: syms\<close> such that 
 \begin{equation}\label{eq:d_imp_c.stepm}
-\<open>Prods G' \<turnstile> [Nt X] \<Rightarrow> \<beta>' \<Rightarrow>(m) map Tm v\<close>
+\<open>Prods G' \<turnstile> [Nt X] \<Rightarrow> \<beta>' \<Rightarrow>(m) map Tm v\<close>.
 \end{equation}
+We now distinguish yet another two cases, now on \<open>m\<close>. \<open>\<turnstile>\<^sub>R\<close> and \<open>\<turnstile>\<^sub>E\<close> denote a reducing and an expanding 
+transition respectively.
 
-We now distinguish yet another two cases, now on \<open>m\<close>. From now on in this proof, instead of 
-@{term \<open>map Tm z\<close>} we occasionally write @{term \<open>z\<close>} for \<open>z :: 't list\<close>. We will also sometimes 
-concatenate lists without an explicit operator, meaning we write @{term \<open>\<alpha> @ \<beta>\<close>} as \<open>\<alpha>\<beta>\<close>. 
-Furthermore, $\<open>\<turnstile>\<^sub>S\<close>$, $\<open>\<turnstile>\<^sub>R\<close>$, and $\<open>\<turnstile>\<^sub>E\<close>$ denote shifting, reducing, and expanding transitions 
-respectively.\par
-
-If \<open>m = 0\<close>, then @{prop \<open>Prods G' \<turnstile> [Nt X] \<Rightarrow> v\<close>}. By Lemma~\ref{completes_Tms} 
-(L\ref{completes_Tms}) we have:
-
+If \<open>m = 0\<close>, then @{prop \<open>Prods G' \<turnstile> [Nt X] \<Rightarrow> v\<close>}. With Lemma~\ref{completes_Tms}
+(L\ref{completes_Tms}) follows:
 \begin{align*}
-&@{term \<open>([A \<rightarrow> \<alpha> \<cdot> \<beta>\<gamma>] # \<rho>, wx)\<close>}\\
+&@{term \<open>([A \<rightarrow> \<alpha> \<cdot> \<beta> @ \<gamma>] # \<rho>, w @ x)\<close>}\\
 &\;\overset{(\ref{d_imp_c.b_decomp(1)}, \ref{d_imp_c.b_decomp(2)}, \ref{d_imp_c.d1u_d2y})}{=\ }
-  \<open>([A \<rightarrow> \<alpha> \<cdot> u @ Nt X # y\<gamma>] # \<rho>, uvyx)\<close>\\
+ @{term \<open>([A \<rightarrow> \<alpha> \<cdot> map Tm u @ Nt X # map Tm y @ \<gamma>] # \<rho>, u @ v @ y @ x)\<close>}\\
 &\;\overset{(L\ref{completes_Tms})}{\<open>\<turnstile>*\<close>\ } 
-  \<open>([A \<rightarrow> \<alpha>u \<cdot> Nt X # y\<gamma>] # \<rho>, vyx)\<close>\\
-&\;\<open>\<turnstile>\<^sub>E ([X \<rightarrow> \<cdot> v] # [A \<rightarrow> \<alpha>u \<cdot> Nt X # y\<gamma>] # \<rho>, vyx)\<close>\\
+  @{term \<open>([A \<rightarrow> \<alpha> @ map Tm u \<cdot> Nt X # map Tm y @ \<gamma>] # \<rho>, v @ y @ x)\<close>}\\
+&\;\<open>\<turnstile>\<^sub>E\<close>\ @{term \<open>([X \<rightarrow> \<cdot> map Tm v] # [A \<rightarrow> \<alpha> @ map Tm u \<cdot> Nt X # map Tm y @ \<gamma>] # \<rho>, v @ y @ x)\<close>}\\
 &\;\overset{(L\ref{completes_Tms})}{\<open>\<turnstile>*\<close>\ }
-  \<open>([X \<rightarrow> v \<cdot> ] # [A \<rightarrow> \<alpha>u \<cdot> Nt X # y\<gamma>] # \<rho>, yx)\<close>\\
-&\;\<open>\<turnstile>\<^sub>R ([A \<rightarrow> \<alpha>u[Nt X] \<cdot> y\<gamma>] # \<rho>, yx)\<close>\\
+  @{term \<open>([X \<rightarrow> map Tm v \<cdot> ] # [A \<rightarrow> \<alpha> @ map Tm u \<cdot> Nt X # map Tm y @ \<gamma>] # \<rho>, y @ x)\<close>}\\
+&\;\<open>\<turnstile>\<^sub>R\<close>\ @{term \<open>([A \<rightarrow> \<alpha> @ map Tm u @ [Nt X] \<cdot> map Tm y @ \<gamma>] # \<rho>, y @ x)\<close>}\\
 &\;\overset{(L\ref{completes_Tms})}{\<open>\<turnstile>*\<close>\ }
-  \<open>([A \<rightarrow> \<alpha>u[Nt X]y \<cdot> \<gamma>] # \<rho>, x)\<close> 
-\overset{(\ref{d_imp_c.b_decomp(1)}, \ref{d_imp_c.d1u_d2y})}{=\ } \<open>([A \<rightarrow> \<alpha>\<beta> \<cdot> \<gamma>] # \<rho>, x)\<close>
+  @{term \<open>([A \<rightarrow> \<alpha> @ map Tm u @ [Nt X] @ map Tm y \<cdot> \<gamma>] # \<rho>, x)\<close>}
+\overset{(\ref{d_imp_c.b_decomp(1)}, \ref{d_imp_c.d1u_d2y})}{=\ } \<open>([A \<rightarrow> \<alpha> @ \<beta> \<cdot> \<gamma>] # \<rho>, x).\<close>
 \end{align*}
-
-Therefore, the implication holds.\par
+Therefore, the implication holds.
 
 Otherwise, if \<open>m = Suc m'\<close> for some \<open>m'\<close>, the derivation @{prop \<open>Prods G' \<turnstile> \<beta>' \<Rightarrow>(m) map Tm v\<close>} can 
 be decomposed as we did before: there exist \<open>\<xi>\<^sub>1, \<xi>\<^sub>2 :: syms\<close>, \<open>Y :: 'n\<close>, \<open>u', v', y' :: 't list\<close>, 
 and \<open>i', j', k' :: nat\<close> such that:
-
 \begin{subequations}
 \begin{gather}
 @{prop \<open>\<beta>' = \<xi>\<^sub>1 @ Nt Y # \<xi>\<^sub>2\<close>}\label{d_imp_c.b'_decomp(1)}\\
 @{prop \<open>v = u' @ v' @ y'\<close>}\label{d_imp_c.b'_decomp(2)}\\
-@{prop \<open>Prods G' \<turnstile> \<xi>\<^sub>1 \<Rightarrow>(i') map Tm u'\<close>}\\
-@{prop \<open>Prods G' \<turnstile> [Nt Y] \<Rightarrow>(j') map Tm v'\<close>}\\
+@{prop \<open>Prods G' \<turnstile> \<xi>\<^sub>1 \<Rightarrow>(i') map Tm u'\<close>}\label{d_imp_c.xi1}\\
+@{prop \<open>Prods G' \<turnstile> [Nt Y] \<Rightarrow>(j') map Tm v'\<close>}\label{d_imp_c.Y}\\
 @{prop \<open>Prods G' \<turnstile> \<xi>\<^sub>2 \<Rightarrow>(k') map Tm y'\<close>}\\
-@{prop \<open>i' + j' + k' = m\<close>}
+@{prop \<open>i' + j' + k' = m\<close>}.
 \end{gather}
 \end{subequations}
 
 This in turn implies that @{prop \<open>i' < n\<close>}, @{prop \<open>j' < n\<close>} and @{prop \<open>k' < n\<close>}, and once again,
-@{prop \<open>Prods G' \<turnstile> [Nt Y] \<Rightarrow>(j') map Tm v'\<close>} implies that @{prop \<open>j' > 0\<close>}, i.e., 
-@{prop \<open>j' = Suc j''\<close>} for some \<open>j''\<close>, meaning this derivation of \<open>v'\<close> is of the form 
-
+\eqref{d_imp_c.Y} implies that @{prop \<open>j' > 0\<close>}, i.e., @{prop \<open>j' = Suc j''\<close>} for some \<open>j''\<close>, 
+meaning this derivation of \<open>v'\<close> is of the form 
 \begin{equation}\label{eq:d_imp_c.stepj''}
-\<open>Prods G' \<turnstile> [Nt Y] \<Rightarrow> \<gamma>' \<Rightarrow>(j'') map Tm v'\<close> \mathrm{\ for\ some\ } \<open>\<gamma>' :: syms\<close>
+\<open>Prods G' \<turnstile> [Nt Y] \<Rightarrow> \<gamma>' \<Rightarrow>(j'') map Tm v'\<close>
 \end{equation}
+for some \<open>\<gamma>' :: syms\<close>. Furthermore, @{prop \<open>j' < n\<close>} implies @{prop \<open>j'' < n\<close>}, and  since 
+\begin{gather}\label{ijk'_less}
+@{prop \<open>i' < n\<close>} \text{, } @{prop \<open>j'' < n\<close>} \text{ and } @{prop \<open>k' < n\<close>}, 
+\end{gather}
+we can use the induction hypothesis (IH) on their corresponding derivations. 
+Let @{term \<open>\<sigma> = [A \<rightarrow> \<alpha> @ map Tm u \<cdot> Nt X # map Tm y @ \<gamma>] # \<rho>\<close>}. The computation then is similar to 
+the previous case, except that
+\[ @{term \<open>([A \<rightarrow> \<alpha> @ map Tm u \<cdot> Nt X # map Tm y @ \<gamma>] # \<rho>, v @ y @ x)\<close>} \] 
+now expands to 
+\[ @{term \<open>([X \<rightarrow> \<cdot> \<xi>\<^sub>1 @ Nt Y # \<xi>\<^sub>2] # \<sigma>, u' @ v' @ y' @ y @ x)\<close>} \]
+by \eqref{eq:d_imp_c.stepm}, \eqref{d_imp_c.b'_decomp(1)} and \eqref{d_imp_c.b'_decomp(2)}.
+By the induction hypothesis, 
+\<open>I\<^sub>G\<close> can then complete \<open>\<xi>\<^sub>1\<close>:
+\[ ... \overset{(IH, \ref{d_imp_c.xi1}, \ref{ijk'_less})}{\<open>\<turnstile>*\<close>\ } 
+@{term \<open>([X \<rightarrow> \<xi>\<^sub>1 \<cdot> Nt Y # \<xi>\<^sub>2] # \<sigma>, v' @ y' @ y @ x)\<close>}, \]
+and now by \eqref{eq:d_imp_c.stepj''}, \<open>I\<^sub>G\<close> expands:
+\[ ...\ \<open>\<turnstile>\<^sub>E\<close>\ @{term \<open>([Y \<rightarrow> \<cdot> \<gamma>'] # [X \<rightarrow> \<xi>\<^sub>1 \<cdot> Nt Y # \<xi>\<^sub>2] # \<sigma>, v' @ y' @ y @ x)\<close>}. \]
+The computation then continues analogously to the first case, applying the IH again to complete 
+\<open>\<gamma>'\<close> and \<open>\<xi>\<^sub>2\<close>. Therefore, the implication also holds in the case where @{prop \<open>j = n\<close>}. 
 
-Since @{prop \<open>i' < n\<close>}, @{prop \<open>j'' < n\<close>} and @{prop \<open>k' < n\<close>}, we can use the Induction Hypothesis
-(IH) on these derivations. We therefore have: 
-
-\begin{align*}
-&@{term \<open>([A \<rightarrow> \<alpha> \<cdot> \<beta>@\<gamma>] # \<rho>, wx)\<close>}\\
-&\;\overset{(\ref{d_imp_c.b_decomp(1)}, \ref{d_imp_c.b_decomp(2)}, \ref{d_imp_c.d1u_d2y})}{=\ }
-  \<open>([A \<rightarrow> \<alpha> \<cdot> u @ Nt X # y\<gamma>] # \<rho>, uvyx)\<close>\\
-&\;\overset{(L\ref{completes_Tms})}{\<open>\<turnstile>*\<close>\ } \<open>([A \<rightarrow> \<alpha>u \<cdot> Nt X # y\<gamma>] # \<rho>, vyx)\<close>\\
-&\;\overset{(\ref{eq:d_imp_c.stepm})}{\<open>\<turnstile>\<^sub>E\<close>\ } \<open>([X \<rightarrow> \<cdot> \<beta>'] # [A \<rightarrow> \<alpha>u \<cdot> Nt X # y\<gamma>] # \<rho>, vyx)\<close>\\
-&\;\overset{(\ref{d_imp_c.b'_decomp(1)}, \ref{d_imp_c.b'_decomp(2)})}{=\ }
-  \<open>([X \<rightarrow> \<cdot> \<xi>\<^sub>1 @ Nt Y # \<xi>\<^sub>2] # [A \<rightarrow> \<alpha>u \<cdot> Nt X # y\<gamma>] # \<rho>, u'v'y'yx)\<close>\\
-&\;\overset{(IH)}{\<open>\<turnstile>*\<close>\ } \<open>([X \<rightarrow> \<xi>\<^sub>1 \<cdot> Nt Y # \<xi>\<^sub>2] # [A \<rightarrow> \<alpha>u \<cdot> Nt X # y\<gamma>] # \<rho>, v'y'yx)\<close>\\
-&\;\overset{(\ref{eq:d_imp_c.stepj''})}{\<open>\<turnstile>\<^sub>E\<close>\ } 
-  \<open>([Y \<rightarrow> \<cdot> \<gamma>'] [X \<rightarrow> \<xi>\<^sub>1 \<cdot> Nt Y # \<xi>\<^sub>2] # [A \<rightarrow> \<alpha>u \<cdot> Nt X # y\<gamma>] # \<rho>, v'y'yx)\<close>\\
-&\;\overset{(IH)}{\<open>\<turnstile>*\<close>\ } \<open>([Y \<rightarrow> \<gamma>' \<cdot>] [X \<rightarrow> \<xi>\<^sub>1 \<cdot> Nt Y # \<xi>\<^sub>2] # [A \<rightarrow> \<alpha>u \<cdot> Nt X # y\<gamma>] # \<rho>, y'yx)\<close>\\
-&\; \<open>\<turnstile>\<^sub>R ([X \<rightarrow> \<xi>\<^sub>1[Nt Y] \<cdot> \<xi>\<^sub>2] # [A \<rightarrow> \<alpha>u \<cdot> Nt X # y\<gamma>] # \<rho>, y'yx)\<close>\\
-&\;\overset{(IH)}{\<open>\<turnstile>*\<close>\ } \<open>([X \<rightarrow> \<xi>\<^sub>1[Nt Y]\<xi>\<^sub>2 \<cdot> ] # [A \<rightarrow> \<alpha>u \<cdot> Nt X # y\<gamma>] # \<rho>, yx)\<close>\\
-&\; \<open>\<turnstile>\<^sub>R ([A \<rightarrow> \<alpha>u[Nt X] \<cdot> y\<gamma>] # \<rho>, yx)\<close>\\
-&\;\overset{(L\ref{completes_Tms})}{\<open>\<turnstile>*\<close>\ }
-  \<open>([A \<rightarrow> \<alpha>u[Nt X]y \<cdot> \<gamma>] # \<rho>, x)\<close> 
-\overset{(\ref{d_imp_c.b_decomp(1)}, \ref{d_imp_c.d1u_d2y})}{=\ } \<open>([A \<rightarrow> \<alpha>\<beta> \<cdot> \<gamma>] # \<rho>, x)\<close>
-\end{align*}
-
-Therefore, the implication also holds in the case where @{prop \<open>j = n\<close>}. We now consider the case 
-where @{prop \<open>j \<noteq> n\<close>}:\par
+Finally, we now consider the case where @{prop \<open>j \<noteq> n\<close>}:
 
 With @{prop \<open>n = i + j + k\<close>} and @{prop \<open>j > 0\<close>}, we know that @{prop \<open>i < n\<close>}, @{prop \<open>j < n\<close>}, and
-@{prop \<open>k < n\<close>} all hold. Therefore, we can use the IH for each of the derivations in the 
-decomposition:
-
-\begin{align*}
-&@{term \<open>([A \<rightarrow> \<alpha> \<cdot> \<beta>\<gamma>] # \<rho>, wx)\<close>}\\
-&\;\<open>= ([A \<rightarrow> \<alpha> \<cdot> \<delta>\<^sub>1 @ Nt X # \<delta>\<^sub>2\<gamma>] # \<rho>, uvyx)\<close>\\
-&\;\overset{(IH)}{\<open>\<turnstile>*\<close>\ } \<open>([A \<rightarrow> \<alpha>\<delta>\<^sub>1 \<cdot> Nt X # \<delta>\<^sub>2\<gamma>] # \<rho>, vyx)\<close>\\
-&\;\overset{(IH)}{\<open>\<turnstile>*\<close>\ } \<open>([A \<rightarrow> \<alpha>\<delta>\<^sub>1 @ [Nt X] \<cdot> \<delta>\<^sub>2\<gamma>] # \<rho>, yx)\<close>\\
-&\;\overset{(IH)}{\<open>\<turnstile>*\<close>\ } \<open>([A \<rightarrow> \<alpha>\<delta>\<^sub>1[Nt X]\<delta>\<^sub>2 \<cdot> \<gamma>] # \<rho>, x) = ([A \<rightarrow> \<alpha>\<beta> \<cdot> \<gamma>] # \<rho>, x)\<close>\\
-\end{align*}
-
-The implication thus holds for all cases and the proof is complete.
+@{prop \<open>k < n\<close>} all hold. Therefore, we can use the IH for each of the derivations \eqref{d_imp_c.d1}, 
+\eqref{d_imp_c.X} and \eqref{d_imp_c.d2} after decomposing \<open>\<beta>\<close> and \<open>w\<close> as we did in the previous
+cases with \eqref{d_imp_c.b_decomp(1)} and \eqref{d_imp_c.b_decomp(2)}. This completes the proof.
 \end{proof}
 \end{lemma}
 
@@ -776,7 +778,7 @@ With this lemma we can finally prove the second direction in the language equiva
 Assume @{prop \<open>w \<in> LangS G\<close>}. Since @{prop \<open>Prods G \<subseteq> Prods G'\<close>}, this implies 
 \[ @{prop \<open>Prods G' \<turnstile> [Nt S] \<Rightarrow>* map Tm w\<close>} \] by the monotonicity of derivations as proved by 
 Nipkow et al. With Lemma~\ref{derives_imp_completes} follows 
-\[ @{prop \<open>([[S' \<rightarrow> \<cdot> [Nt S]]], w) \<turnstile>* ([[S' \<rightarrow> [Nt S] \<cdot> ]], [])\<close>} \] 
+\[ @{prop \<open>([[S' \<rightarrow> \<cdot> [Nt S]]], w) \<turnstile>* ([[S' \<rightarrow> [Nt S] \<cdot> ]], [])\<close>}. \] 
 
 This is equivalent to @{prop \<open>w \<in> gpda.Lang I\<^sub>G\<close>}.
 \end{proof}
@@ -790,27 +792,108 @@ And thus with Lemma~\ref{ipda.Lang_subst_Lang_G}:
 \end{theorem}
 
 We have now defined a nondeterministic GPDA that works with items and accepts exactly its underlying 
-language. As a final remark, it is worth pointing out that our proof differs somewhat from that of 
-Wilhelm et al. Rather than of Lemma~\ref{derives_imp_completes}, they prove a special case thereof, 
-namely the statement
+language. With this IPDA definition, we can see one of the benefits of extending \<open>G\<close>: if we were to 
+define the set of final states to be the set of all complete items of the form @{term \<open>[S \<rightarrow> \<alpha> \<cdot> ]\<close>},
+the automaton could encounter a final state before the end of a computation. Since \<open>S'\<close> is in not 
+on the RHS of any production, this scenario can not occur after the extension.\par
+
+As a final remark, it is worth pointing out that our proof differs somewhat from that of
+Wilhelm et al. Rather than of Lemma~\ref{derives_imp_completes}, they prove a special case 
+thereof~\cite[p. 61]{Wilhelm}, namely the statement
 \begin{quote}
-For each derivation \<open>Prods G \<turnstile> [Nt A] \<Rightarrow> \<alpha> \<Rightarrow>* map Tm w\<close>, 
-\mbox{@{prop \<open>([A \<rightarrow> \<cdot> \<alpha>] # \<rho>, w @ v) \<turnstile>* ([A \<rightarrow> \<alpha> \<cdot> ] # \<rho>, v)\<close>}} for arbitrary \<open>\<rho> :: item list\<close> and 
-\<open>v :: 't list\<close>.
+\textit{For each derivation \<open>Prods G \<turnstile> [Nt A] \<Rightarrow> \<alpha> \<Rightarrow>* map Tm w\<close> with \<open>A :: 'n\<close>, 
+\[ @{prop \<open>([A \<rightarrow> \<cdot> \<alpha>] # \<rho>, w @ v) \<turnstile>* ([A \<rightarrow> \<alpha> \<cdot> ] # \<rho>, v)\<close>} \] 
+for arbitrary \<open>\<rho> :: item list\<close> and \<open>v :: 't list\<close>.}
 \end{quote}
 
 However, this statement is too weak, as we will soon need the stronger lemma we have proved instead.\<close>
 
 section \<open>The Characteristic Finite Automaton and the Canonical LR(0) Automaton\<close>
-
 (*<*)
 end
 context Extended_Cfg
-begin       
+begin
+
+notation (latex output) char_fa
+  (\<open>\<^latex>\<open>\ensuremath{\mathrm{char}(G)}\<close>\<close>)
 (*>*)
 
 text \<open>In this section, we will show the relation between rightmost derivations and the IPDA in more 
 detail, as well as the define finite automata that the canonical LR(0) parser will operate with.\<close>
+
+text\<open>In order to construct our parser, we will first define an automaton that can determine possible
+reductions. We again define a nondeterministic automaton, in this case an NFA, that we will call the  
+\concept{characteristic finite automaton} to \<open>G\<close>. We base our finite automata on the formalization
+thereof by Paulson~\<^cite>\<open>Paulson\<close>.
+
+\begin{definition}[Characteristic finite automaton]
+The characteristic finite automaton to \<open>G\<close> is the @{typ \<open>(('n, 't) sym, ('n, 't) item) nfa\<close>}:
+\begin{multline*}
+  @{const char_fa} = \<open>\<lparr>nfa.states = It G', init = {[S' \<rightarrow> [] \<cdot> [Nt S]]},\<close>\\
+  \<open>final = completes (It G'), nxt = \<Delta>, eps = \<E>\<rparr>\<close>
+\end{multline*}
+with
+% Fix style?
+@{term [display, margin = 80] \<open>\<Delta>(q, a) = (case q of [X \<rightarrow> \<alpha> \<cdot> Y # \<beta>] \<Rightarrow> 
+  if a = Y \<and> (X, \<alpha>@Y#\<beta>) \<in> Prods G' then {[X \<rightarrow> \<alpha>@[Y] \<cdot> \<beta>]}
+  else {} | _ \<Rightarrow> {})\<close>}
+and
+\begin{multline*}
+\<open>\<E> = {([X \<rightarrow> \<alpha> \<cdot> Nt Y # \<beta>], [Y \<rightarrow> [] \<cdot> \<gamma>])\<close>\\
+  \<open>| X \<alpha> Y \<beta> \<gamma>. (X, \<alpha> @ Nt Y # \<beta>) \<in> Prods G' \<and> (Y, \<gamma>) \<in> Prods G'}\<close>
+\end{multline*}
+\end{definition}
+
+The characteristic finite automaton can therefore perform shifting and expanding transitions akin to 
+those of the IPDA @{const ipda.I\<^sub>G}. The inability of @{const char_fa} of performing reducing 
+transitions is compensated by the fact that it is able to shift nonterminals as well as terminals. 
+@{const char_fa} can therefore reach an item in @{term \<open>It G\<close>} by read the concatenation of prefixes 
+leading to this particular item, as explained by Wilhelm et al.~\cite[p. 103]{Wilhelm}
+
+We will now work towards showing certain equivalences between @{const char_fa} computations, rightmost 
+derivations, and @{const ipda.I\<^sub>G} computations.\<close>
+
+subsection \<open>Rightmost Chains\<close>
+
+text \<open>Wilhelm et al. informally assert that for a rightmost derivation 
+\<open>Prods G' \<turnstile> [Nt S'] \<Rightarrow>r* \<gamma>' @ Nt A # map Tm w \<Rightarrow>r \<gamma>' @ \<alpha> @ \<beta> @ map Tm w\<close>, there exists a decomposition
+of the form
+\begin{equation}\label{WSH rm chain}
+\begin{split}
+\<open>Prods G'\<close>\ & \<open>\<turnstile> [Nt S'] \<Rightarrow>r \<alpha>\<^sub>1 @ Nt X\<^sub>1 # \<beta>\<^sub>1 \<Rightarrow>r* \<alpha>\<^sub>1 @ Nt X\<^sub>1 # map Tm v\<^sub>1\<close>\\
+        & \<open>\<Rightarrow>r \<alpha>\<^sub>1\<alpha>\<^sub>2 @ Nt X\<^sub>2 # \<beta>\<^sub>2 @ map Tm v\<^sub>1\<close>\\ 
+        & \<open>\<Rightarrow>r* ... \<Rightarrow>r* \<alpha>\<^sub>1\<alpha>\<^sub>2 ... \<alpha>\<^sub>n @ Nt X\<^sub>n # map Tm (v\<^sub>n ... v\<^sub>2v\<^sub>1)\<close>\\
+        & \<open>\<Rightarrow>r (\<alpha>\<^sub>1 ... \<alpha>\<^sub>n) \<alpha>\<beta> @ map Tm (v\<^sub>n ... v\<^sub>1)\<close>.
+\end{split}
+\end{equation}
+where \<open>X\<^sub>n = A\<close> and terms such as \<open>\<alpha>\<^sub>1\<alpha>\<^sub>2\<close>, \<open>\<alpha>\<beta>\<close>, or \<open>v\<^sub>2v\<^sub>1\<close> denote the concatenation of the individual 
+\<open>\<alpha>\<^sub>1, \<alpha>\<^sub>2, \<alpha>, \<beta> :: syms\<close>, and  \<open>v\<^sub>2, v\<^sub>1 :: 't list\<close>. 
+
+We will now formalize this concept by defining \concept{rightmost chains} inductively. If sentential 
+form \<open>\<alpha>\<close> reaches sentential form \<open>\<beta>\<close> with rightmost chain \<open>\<rho>\<close> under production set \<open>P\<close>, we write 
+@{prop \<open>P \<turnstile> \<alpha> \<midarrow>\<rho>\<rightarrow>r* \<beta>\<close>}. We define the following rules for some fixed \<open>P\<close>:
+\begin{itemize}
+\item @{thm rm_chain.refl} 
+\item 
+@{thm [mode=Rule] rm_chain.step}
+\end{itemize}
+
+\begin{example}
+By our definition of rightmost chains, we would write \eqref{WSH rm chain} as
+\begin{equation*}
+\begin{split}
+\<open>P \<turnstile> [Nt S']\<close> & \<open>\<midarrow>[\<close>X_{n-1} \<open>\<rightarrow> \<alpha>\<^sub>n \<cdot> Nt X\<^sub>n # \<beta>\<^sub>n] #\<close> \cfitem{X_{n-2}}{\alpha_{n-1}}{Nt X_{n-1} 
+  \# \beta_{n-1}}\\
+              & 
+\begin{multlined}
+\# ... \<open># [S' \<rightarrow> \<alpha>\<^sub>1 \<cdot> Nt X\<^sub>1 # \<beta>\<^sub>1] # []\<rightarrow>\<close>\\ 
+  \<open>\<alpha>\<^sub>1 @ \<alpha>\<^sub>2 @ \<sigma> \<alpha>\<^sub>n @ Nt X\<^sub>n # map Tm (v\<^sub>n @ ... @ v\<^sub>2 @ v\<^sub>1)\<close>.
+\end{multlined}
+\end{split}
+\end{equation*}
+\end{example}
+
+\<close>
 
 
 
